commit mid work

current_files/current.v
@@ -9,13 +9,436 @@ From mathcomp Require Import order.
 Require Import Streams.
 From HB Require Import structures.
 From deriving Require Import deriving.
-Require Import Stdlib.Program.Equality.
+Require Import Coq.Program.Equality.
 From Equations Require Import Equations.
-Require Import Stdlib.Classes.DecidableClass.
-From Stdlib Require Eqdep.
-
+Require Import Coq.Classes.DecidableClass.
 Import Order.TTheory.
 Open Scope order_scope.
 
-Require Export NonInterference.llmwork.theorems.
+Require Import NonInterference.theorems.
 
+Definition inl_some {A B : Set} (x : A + B) := if x is inl x' then Some x' else None.
+Definition inr_some {A B : Set} (x : A + B) := if x is inr x' then Some x' else None.
+Definition option_inl_some {A B : Set} (x : option (A + B)) := if x is Some (inl x') then Some x' else None.
+Definition inr_inl_some {A B C : Set} (x : A + (B + C)) := if x is inr (inl x') then Some x' else None.
+Definition inr_inr_some {A B C : Set} (x : A + (B + C)) := if x is inr (inr x') then Some x' else None.
+Definition is_none (A : Set) (x : option A) := if x is None then true else false.
+Definition is_some (A : Set) (x : option A) := if x is Some _ then true else false.
+Definition some_inl (A B : Set) (x : option (A + B)) : option A := if x is Some (inl x') then Some x' else None.
+
+Fixpoint sum_N n (f : nat -> Ty) : Ty :=
+  let t := f n in
+  match n with
+  | 0 => t
+  | S n' => Sum t (sum_N n' f)
+  end.
+
+Fixpoint times_N n (f : nat -> Ty) : Ty :=
+  let t := f n in
+  match n with
+  | 0 => t
+  | S n' => Times t (times_N n' f)
+  end.
+
+Definition map_option (A B : Set) (f : A -> B) (x : option A) : option B := if x is Some x' then Some (f x') else None.
+Definition map_sum {A B C D :Set} (f : A -> C) (g : B -> D) := fun (x: A + B) => match x with
+                                                                                | inl x' => inl (f x')
+                                                                                | inr x' => inr (g x')
+                                                                                 end.
+Definition map_pair {A B C D :Set} (f : A -> C) (g : B -> D) := fun (x: A * B) => match x with
+                                                                                | (x0,x1) => (f x0, g x1)
+                                                                                  end.
+Definition times_Option_n (n : nat) (f : nat -> Ty) := times_N n (Option \o f).
+
+(*Example*)
+Definition my_f_I := fun (n : nat) => match n with
+                                      | 0 => TInterrupt (*handler*)
+                                      | 1 => THandlerOutput (*private*)
+                                      | 2 => Unit (*public*)
+                                      | 3 => TInterrupt (*scheduler*)
+                                      | _ => Unit
+                                      end.
+
+Definition my_f_O := fun (n : nat) => match n with
+                                      | 0 => THandlerOutput
+                                      | 1 => TTypeSyscall
+                                      | 2 => TPublicOutput
+                                      | 3 => Nat
+                                      | _ => Unit
+                                      end.
+Definition my_T_in := Sum Unit TInterrupt. (*We need Unit input to be able to differentiate trace, otherwise we only have interrupts in the trace*)
+Definition my_T_out := Option (Sum TPublicOutput TTypeSyscall).
+Definition my_T_in' := Times (Times Nat Nat) (times_Option_n 3 my_f_I).
+Definition my_T_out' := times_Option_n 3 my_f_O.
+
+
+(*Process*)
+
+Definition alternate_generic (A B C: Ty) (x y : [B]) (z : [C]) := @map _ (Sum _ _) (Sum _ (Times Bool C)) B 
+                        inl
+                        (fun o => if o is inr (true,z) then x else y)
+                        (@loop (Sum A (Times Bool C))
+                        (@map (Sum A _) _ _ (Sum _ _) id (fun o => inr o)
+                        ((@sta (Sum _ _) _ Bool
+                           (fun i v => if i is inl _ then true else false)
+                           (fun o v => v)
+                           false
+                           (@out (Times Bool _ ) C z)
+                        )))).
+
+Definition alternate_generic2 (A B C : Ty) (x y : [B]) (z : [C]) (pred : [A] -> bool) :=
+  @map _ (Sum _ _) (Sum _ (Times Bool C)) B 
+                        inl
+                        (fun o => if o is inr (true,z) then x else y)
+                        (@loop (Sum A (Times Bool C))
+                        (@map (Sum A _) _ _ (Sum _ _) id (fun o => inr o)
+                        ((@sta (Sum _ _) _ Bool
+                           (fun i v => match i with | inl i' => v || pred i' | _ => false end)
+                           (fun o v => v)
+                           false
+                           (@out (Times Bool _ ) C z)
+                        )))).
+
+Definition scheduled_process_pool
+  (n : nat)
+  (f_coopt : nat -> bool)
+  (f_initial : nat -> bool)
+  (f_I f_O : nat -> Ty)
+  (f_proc : forall n, Proc (f_I n) (f_O n)) : Proc (Times (Times Nat Nat) ((times_Option_n n f_I))) (times_Option_n n f_O).
+  elim: n.
+  - simpl.
+    eapply map. simpl.
+      instantiate (1:= Times Bool (Option (f_I 0))). exact (fun n => ((0.+1 \in [:: fst (fst n); snd (fst n)],snd n))).
+      exact id. 
+    eapply swi. exact (f_initial 0.+1). 
+    eapply maybe. 
+    eapply map.
+      eapply id. 
+      exact (fun o => (f_coopt 0.+1,o)).
+    exact (f_proc 0).
+
+  - intros. simpl.
+    eapply par.
+    * eapply map.
+      instantiate (1:= Times Bool (Option (f_I n.+1))). simpl.
+      exact (fun x => ((n.+2) \in [:: fst (fst x); snd (fst x)], fst (snd x))).
+        exact id. 
+      eapply swi.
+        exact (f_initial n.+2). 
+      eapply maybe.
+      eapply map.
+        exact id.     
+        exact (fun o => (f_coopt n.+2,o)).
+      (*eapply maybe.*) (*not necessary anymore*)
+      exact (f_proc n.+1).
+    * eapply map. 3: apply H. simpl. 
+      exact (map_pair id snd).
+      exact id. 
+Defined.
+
+Definition inr_or_def {A B : Set} (def: B) (x : A + B) := if x is inr x' then x' else def.
+
+Definition only_loop
+  (T_in' T_out' : Ty)   
+  (f_route : [T_out'] -> [T_in'])
+  (def : [T_out'])
+  (p : Proc T_in' T_out')
+  : Proc T_in' T_out' :=
+  (@map T_in' (Sum T_in' T_out') (Sum T_in' T_out') T_out' inl (inr_or_def def)
+                          (@loop (Sum T_in' T_out')
+                             (@map (Sum T_in' T_out')
+                                    T_in'
+                                    _
+                                    (Sum _ _)
+                                (fun i  =>
+                                   match i with
+                                   | inl i' => i'
+                                   | inr o  => f_route o (*i tilfælde hvor vi både ændrer switch og rerouter input, problem?*)
+                                   end) inr
+                                p))).
+
+Definition low_p := @out Unit TPublicOutput GetRequest.
+Definition handler := @alternate_generic TInterrupt THandlerOutput Unit2 Notify Nothing tt.
+Definition high_p := @alternate_generic2 THandlerOutput TTypeSyscall Unit1 Syscall NOP tt (fun i => i == Notify).
+
+(*
+From:
+
+private on ->(?timerinterrupt)
+private on, scheduler on ->(!(handler_index,private_out))
+handler on ->(!handler_out)
+scheduler on ->(!public_index)
+public on ->(?timerinterrupt)
+public on, scheduler on ->(!(handler_index,public_out))
+handler on ->(!handler_out)
+scheduler on ->(!private_index)
+...
+
+
+To:
+
+private on ->(?timerinterrupt)
+private on ->(!private_out)
+scheduler on ->(!handler_index)
+handler on ->(!handler_out)
+scheduler on ->(!public_index)
+public on ->(?timerinterrupt)
+public on ->(!public_out)
+scheduler on ->(!handler_index)
+handler on ->(!handler_out)
+scheduler on ->(!private_index)
+...
+ *)
+Definition good_schedulerp :  Proc TInterrupt Nat.
+  eapply map. apply id. instantiate (1:= Times Bool Unit).
+  exact (fun o => if fst o then 3 else 2).
+  eapply (@sta _ _ Bool).
+  - exact (fun ih b => match ih with | TimerInterrupt => ~~ b | DiskInterrupt => b end).
+  - exact (fun _ b => b).
+  - exact false.
+  - eapply out. con.
+Defined.
+
+(* Definition sstream := Stream ([(Sum TInterrupt THandlerOutput)] + [(Times Nat Nat)]).
+
+Definition my_sstreamF (s : sstream) := Cons (inl (inl TimerInterrupt)) (Cons (inr (2,1)) (Cons (inl (inr Nothing)) (Cons (inr (3,3))
+                                                                                                                      (Cons (inl (inl TimerInterrupt)) (Cons (inr (3,1)) (Cons (inl (inr Nothing)) (Cons (inr (2,2)) s))))))).
+
+CoFixpoint my_sstream := my_sstreamF my_sstream.
+
+Lemma my_sstream_eq : my_sstream = my_sstreamF my_sstream.
+Proof.
+rewrite {1}/my_sstream.
+rewrite {1}(coseq_match (cofix my_sstream : sstream := my_sstreamF my_sstream)).
+simpl.
+rewrite /my_sstreamF.
+do ? f_equal.
+Qed. *)
+
+(*Lemma schedulerp_trace : trace my_sstream good_schedulerp.
+Proof.
+  pcofix CIH.
+  rewrite my_sstream_eq /my_sstreamF /good_schedulerp.
+  bundle;left.
+  bundle;left.
+  bundle;left.
+  bundle;left.
+  bundle;left.
+  bundle;left.
+  bundle;left.
+  bundle;right.
+Qed.*)
+
+
+Definition unit_p : Proc Unit Unit := @out Unit Unit tt.
+
+Definition my_procs_good : forall n, Proc (my_f_I n) (my_f_O n).
+  case. apply handler.
+  case. apply high_p.
+  case. apply low_p.
+  case. simpl. apply good_schedulerp.
+  elim. apply unit_p.
+  intros. apply unit_p.
+Defined.
+Definition my_f_coopt n := n == 4.
+Definition my_f_initial n := n == 2.
+Definition process_pool_good := @scheduled_process_pool 3 my_f_coopt my_f_initial my_f_I my_f_O my_procs_good.
+
+
+Definition LoopType_n (n : nat) (f_I f_O : nat -> Ty) := Sum (times_Option_n n f_I) (times_Option_n n f_O).
+Definition None_N (n : nat) (f_O : nat -> Ty) : [(times_Option_n n f_O)].
+elim: n. simpl. exact None.
+intros. simpl. eapply pair. exact None. exact H.
+Defined.
+Definition collapse_in_out (n : nat) (f_I f_O : nat -> Ty) (x : [LoopType_n n f_I f_O]) : [times_Option_n n f_O]  :=
+  match x with
+  | inl _ => None_N n f_O
+  | inr x' => x'
+  end.
+Definition my_def := None_N 3 my_f_O.
+Definition none4 : [ (times_Option_n 3 my_f_I) ]  := (None,(None,(None,None))).
+Definition my_f_route_good (t : [my_T_out']) : [my_T_in'] :=
+  match t with
+  | (Some sch,_) => ((sch, sch),none4)
+  | (_ ,(Some publ, _)) => ((0,0),none4)
+  | (_ ,(None,(Some prv,_))) => ((0,0),none4)
+  | (_ ,(None,(None,Some handl))) => ((1,4),(None,(None,(Some handl,None)))) (*(1,4) = turn off yourself, turn on scheduler*)
+  | _ => ((0,0),none4)    
+  end.
+Definition my_f_in_sch_good (t : [my_T_in]) : [Times Nat Nat] := match t with | inl tt | inr DiskInterrupt => (0,0) | inr TimerInterrupt => (0,4) end.
+Definition my_f_in_t (t : [my_T_in]) : [ (times_Option_n 3 my_f_I) ] := match t with
+                                                                        | inl tt => (None,(Some tt,(None,None)))
+                                                                        | inr TimerInterrupt => (Some TimerInterrupt,(None,(None,None)))
+                                                                        | inr DiskInterrupt => (None,(None,(None,Some DiskInterrupt))) end.
+Definition my_f_in_good (t : [my_T_in]) : [my_T_in'] := (my_f_in_sch_good t, my_f_in_t t).
+Definition my_f_out (t : [my_T_out']) := match t with
+                                         | (_,(Some p,(None,None))) => Some (inl p)
+                                         | (_,(None,(Some sys,None))) => Some (inr sys)
+                                         | _ => None
+                                         end.
+
+(* V_state represents the CPU/OS internal state registers, combining:
+   1. (timer_received, disk_received) : Latch registers that record when an interrupt
+      signal is active on the bus during the current step.
+   2. (timer_pending, disk_pending)   : Checked at the end of the CPU cycle (on output)
+      to trigger preemption/switching for the *next* step.
+   3. (p_sched, handler_active)       : Tracks which process has been scheduled by the OS (single Nat),
+      and whether the interrupt handler is currently active. *)
+Definition V_state := Times (Times (Times Bool Bool) (Times Bool Bool)) (Times Nat Bool).
+
+(* Filters out scheduler and handler interrupt inputs from the input tuple,
+   preventing them from leaking or causing premature process activation during
+   normal process execution steps. *)
+Definition clear_interrupts (i : [times_Option_n 3 my_f_I]) : [times_Option_n 3 my_f_I] :=
+  (None, (fst (snd i), (fst (snd (snd i)), None))).
+
+(* f_state is the state transition function on INPUT (inl transition).
+   It latches incoming interrupt signals (TimerInterrupt or DiskInterrupt)
+   into the timer_received and disk_received registers. The currently executing
+   process is unaffected and completes its step. *)
+Definition f_state (i_in' : [my_T_in']) (v : [V_state]) : [V_state] :=
+  let i_pool := snd i_in' in
+  let timer_rec := if fst i_pool is Some TimerInterrupt then true else fst (fst (fst v)) in
+  let disk_rec  := if snd (snd (snd i_pool)) is Some DiskInterrupt then true else snd (fst (fst v)) in
+  ((timer_rec, disk_rec), snd (fst v), snd v).
+
+(* g_state is the state transition function on OUTPUT (inr transition).
+   It updates the CPU registers at the end of each CPU cycle (step boundary):
+   - If the scheduler ran: it updates the next scheduled process (p_sched) to the single Nat,
+     clears the timer pending/received flags, and turns on the handler_active flag
+     if a disk interrupt is pending and requires handling.
+   - If the handler ran: it clears handler_active and the disk pending/received flags.
+   - If a normal process ran: it promotes latched interrupts (timer_received/disk_received)
+     to pending flags (timer_pending/disk_pending) to trigger context switches next. *)
+Definition g_state (o : [my_T_out']) (v : [V_state]) : [V_state] :=
+  let timer_received := fst (fst (fst v)) in
+  let disk_received  := snd (fst (fst v)) in
+  let timer_pending  := fst (snd (fst v)) in
+  let disk_pending   := snd (snd (fst v)) in
+  let p_sched        := fst (snd v) in
+  let handler_active := snd (snd v) in
+  
+  match fst o with
+  | Some p_next =>
+      (* Scheduler ran! *)
+      let timer_pending' := false in
+      let timer_received' := false in
+      let p_sched' := p_next in
+      let handler_active' := disk_pending in
+      let disk_pending' := if disk_pending then false else disk_pending in
+      let disk_received' := if disk_pending then false else disk_received in
+      ((timer_received', disk_received'), (timer_pending', disk_pending'), (p_sched', handler_active'))
+  | None =>
+      match snd (snd (snd o)) with
+      | Some _ =>
+          (* Handler ran! *)
+          let handler_active' := false in
+          let disk_pending' := false in
+          let disk_received' := false in
+          ((timer_received, disk_received'), (timer_pending, disk_pending'), (p_sched, handler_active'))
+      | None =>
+          (* Normal process ran! *)
+          let timer_pending' := if timer_received then true else timer_pending in
+          let disk_pending'  := if disk_received then true else disk_pending in
+          let timer_received' := false in
+          let disk_received'  := false in
+          ((timer_received', disk_received'), (timer_pending', disk_pending'), (p_sched, handler_active))
+      end
+  end.
+
+Definition I_pool := times_Option_n 3 my_f_I.
+
+(* override_pool_input maps the stateful registers to pool-level execution flags:
+   - If timer_pending is set: we preempt the running process, activate the scheduler (index 4),
+     and feed it the TimerInterrupt.
+   - If handler_active is set: we preempt the running process, activate the handler (index 1),
+     and feed it the DiskInterrupt.
+   - Otherwise: the normal scheduled process (p_sched) is executed as (p_sched, p_sched), and
+     interrupt inputs are cleared. *)
+Definition override_pool_input (x : [Times V_state my_T_in']) : [Times (Times Nat Nat) I_pool] :=
+  let v := fst x in
+  let i_in' := snd x in
+  let i_pool := snd i_in' in
+  let timer_pending := fst (snd (fst v)) in
+  let disk_pending  := snd (snd (fst v)) in
+  let p_sched        := fst (snd v) in
+  let handler_active := snd (snd v) in
+  
+  if timer_pending then
+    ((0, 4), (Some TimerInterrupt, (None, (None, None))))
+  else if handler_active then
+    ((0, 1), (None, (None, (None, Some DiskInterrupt))))
+  else
+    ((p_sched, p_sched), clear_interrupts i_pool).
+
+Definition v_state_init : [V_state] :=
+  ((false, false), (false, false), (2, false)).
+
+Definition my_only_loop_good_inner : Proc my_T_in' my_T_out'.
+  eapply (@map my_T_in' my_T_in' (Times V_state my_T_out') my_T_out'). exact id. exact (fun x => snd x).
+  eapply (@sta _ _ V_state).
+  - exact f_state.
+  - exact g_state.
+  - exact v_state_init.
+  - eapply map.
+    + exact override_pool_input.
+    + exact id.
+    + exact process_pool_good.
+Defined.
+
+Definition my_only_loop_good' := @only_loop my_T_in' my_T_out' my_f_route_good my_def my_only_loop_good_inner.
+
+Definition my_only_loop_good : Proc my_T_in my_T_out .
+  eapply map. apply my_f_in_good. apply my_f_out. apply my_only_loop_good'.
+Defined.
+
+  
+
+Definition out0 x : [my_T_out'] := (Some x,(None,(None,None))).
+Definition out1 x : [my_T_out'] := (None,(Some x,(None,None))).
+Definition out2 x : [my_T_out'] := (None,(None,(Some x,None))).
+Definition out3 x : [my_T_out'] := (None,(None,(None, Some x))).
+
+(*Spec for good scheduler*)
+(*Add diskinterrupt*)
+Definition seqtype' := seq ([my_T_in'] + [my_T_out']).
+Definition newtrace' : seqtype' :=
+  cons (inl (my_f_in_good (inr TimerInterrupt)))
+  (cons (inr (None, (None, (Some NOP, None))))
+  (cons (inr (out0 3))
+  (cons (inr (out1 GetRequest))
+  (cons (inl (my_f_in_good (inr DiskInterrupt)))
+  (cons (inr (out1 GetRequest))
+  (cons (inl (my_f_in_good (inr TimerInterrupt)))
+  (cons (inr (out1 GetRequest))
+  (cons (inr (out0 2))
+  (cons (inr (out3 Notify))
+  (cons (inr (out2 Syscall)) nil)))))))))).
+
+Definition seqtype := seq ([my_T_in] + [my_T_out]).
+
+Definition newtrace_wrap : seqtype  :=
+  cons (inl (inr TimerInterrupt))
+  (cons (inr (Some (inr NOP)))
+  (cons (inr None)
+  (cons (inr (Some (inl GetRequest)))
+  (cons (inl (inr DiskInterrupt))
+  (cons (inr (Some (inl GetRequest)))
+  (cons (inl (inr TimerInterrupt))
+  (cons (inr (Some (inl GetRequest)))
+  (cons (inr None)
+  (cons (inr None)
+  (cons (inr (Some (inr Syscall))) nil)))))))))).
+
+Ltac rewr ::= rewrite /low_p /handler /high_p /only_loop /my_only_loop_good' /my_only_loop_good /process_pool_good /good_schedulerp /my_f_coopt /scheduled_process_pool /high_p /alternate_generic /alternate_generic2 /low_p.
+
+Lemma newtrace'_trace : Trace (eqpair_LR (eqmaybe (publicRel Nat))
+                          (eqpair_LR (eqmaybe (publicRel TPublicOutput))
+                             (eqpair_LR (eqmaybe (semiprivateRel TTypeSyscall))
+                                (eqmaybe (semiprivateRel THandlerOutput))))) false newtrace' my_only_loop_good'.
+Proof.
+Admitted.
+
+Lemma newtrace_trace : Trace (eqmaybe (eqsum_LR (publicRel TPublicOutput) (semiprivateRel TTypeSyscall))) false newtrace_wrap my_only_loop_good.
+Proof.
+Admitted.
