process.v
@@ -12,1968 +12,448 @@ From deriving Require Import deriving.
 Require Import Coq.Program.Equality.
 From Equations Require Import Equations.
 Require Import Coq.Classes.DecidableClass.
-
 Import Order.TTheory.
 Open Scope order_scope.
 
-(*Before*)
-(*Parameter (level : tbLatticeType (Order.Disp tt tt)).*)
+Require Import NonInterference.theorems.
 
-(*Just for now*)
-Definition level := bool.
+Definition inl_some {A B : Set} (x : A + B) := if x is inl x' then Some x' else None.
+Definition inr_some {A B : Set} (x : A + B) := if x is inr x' then Some x' else None.
+Definition option_inl_some {A B : Set} (x : option (A + B)) := if x is Some (inl x') then Some x' else None.
+Definition inr_inl_some {A B C : Set} (x : A + (B + C)) := if x is inr (inl x') then Some x' else None.
+Definition inr_inr_some {A B C : Set} (x : A + (B + C)) := if x is inr (inr x') then Some x' else None.
+Definition is_none (A : Set) (x : option A) := if x is None then true else false.
+Definition is_some (A : Set) (x : option A) := if x is Some _ then true else false.
+Definition some_inl (A B : Set) (x : option (A + B)) : option A := if x is Some (inl x') then Some x' else None.
 
-Ltac con := constructor.
-Ltac econ := econstructor.
-Ltac inv H := inversion H;subst.
-Ltac econs := try do ? econ; done.
-                     
-Ltac split_ando :=
-  intros;
-   repeat
-    match goal with
-    | H:is_true (_ && _) |- _ => destruct (andP H); clear H    | H:_ && _ = true |- _ => destruct (andP H); clear H
-    | H:_ /\ _ |- _ => destruct H
-    | |- _ /\ _ => con
-    | |- is_true (_ && _) => apply /andP ; con
-    | |- is_true (_ || _) => apply /orP
-    | H : ex _ |- _ => destruct H
-    end; auto.
-
-
-Ltac split_and :=
-  intros;
-   repeat
-    match goal with
-    | H:is_true (_ && _) |- _ => destruct (andP H); clear H
-    | H:_ && _ = true |- _ => destruct (andP H); clear H
-    | H:_ /\ _ |- _ => destruct H
-    | |- _ /\ _ => con
-    | |- is_true (_ && _) => apply /andP ; con
-    | H : ex _ |- _ => destruct H
-    end; auto;subst.
-
-
-Ltac ssa' := rewrite ?inE;simpl in *; split_and;try done.
-Ltac ssa := rewrite ?inE;simpl in *; split_ando;try done.
-
-Ltac de i := destruct i;ssa.
-
-Ltac case_if := match goal with 
-                | [ |- context[if ?X then _ else _ ]] => have : X by subst
-                | [ |- context[if ?X then _ else _ ]] => have : X = false by subst 
-
-                | [ |- context[if ?X then _ else _ ]] => let H := fresh in destruct X eqn:H
-
-                end; try (move=>->).
-
-Lemma coseq_match : forall {A : Type} (g : Stream A), g = match g with | Cons a b => Cons a b end.  
-Proof. move => A[] //=. Qed. 
-
-Ltac coseq_tac l := rewrite (coseq_match l) /=. 
-Ltac coseq_tac_in l H := rewrite (coseq_match l) /= in H.
-
-Definition order (b1 b2 : level) := b1 <= b2.
-
-Record myrel (A : Set) :=
-        MyRel {
-           dis : level -> A -> Prop;
-           rel : level -> A -> A -> Prop;
-           equiv : forall l, Equivalence (rel l);
-           _ : forall l0 l1, order l0 l1 ->
-                             forall a0 a1, rel l1 a0 a1 -> rel l0 a0 a1;
-           _ : forall l0 l1, order l0 l1 ->
-                             forall a, dis l1 a -> dis l0 a;
-           _: forall l a0, dis l a0 -> forall a1, dis l a1 <-> rel l a0 a1 (* dis is an equivalence class: (->) contains enough, (<-) does not include too much s  *)
-(*           _: forall l a0 a1, dis l a0 -> rel l a0 a1 -> dis l a1;
-           _: forall l a0 a1, dis l a0 -> dis l a1 -> rel l a0 a1*)
-          }.
-
-(*Existing Class myrel. 
-Hint Mode myrel +.*)
-
-(* Types *)
-
-(*Example 3*)
-Inductive Interrupt := DiskInterrupt | TimerInterrupt.
-Inductive HandlerOutput := Nothing | Notify.
-Inductive TypeSyscall := Syscall | NOP.
-Inductive PublicOutput := GetRequest | Public_NOP.
-Inductive PublicInput := PublicIn
-.
-Definition Interrupt_indDef := [indDef for Interrupt_rect].
-Canonical Interrupt_indType := IndType Interrupt Interrupt_indDef.
-Definition Interrupt_hasDecEq := [derive hasDecEq for Interrupt].
-HB.instance Definition _ := Interrupt_hasDecEq.
-
-Definition HandlerOutput_indDef := [indDef for HandlerOutput_rect].
-Canonical HandlerOutput_indType := IndType HandlerOutput HandlerOutput_indDef.
-Definition HandlerOutput_hasDecEq := [derive hasDecEq for HandlerOutput].
-HB.instance Definition _ := HandlerOutput_hasDecEq.
-
-Definition TypeSyscall_indDef := [indDef for TypeSyscall_rect].
-Canonical TypeSyscall_indType := IndType TypeSyscall TypeSyscall_indDef.
-Definition TypeSyscall_hasDecEq := [derive hasDecEq for TypeSyscall].
-HB.instance Definition _ := TypeSyscall_hasDecEq.
-
-Definition PublicOutput_indDef := [indDef for PublicOutput_rect].
-Canonical PublicOutput_indType := IndType PublicOutput PublicOutput_indDef.
-Definition PublicOutput_hasDecEq := [derive hasDecEq for PublicOutput].
-HB.instance Definition _ := PublicOutput_hasDecEq.
-
-Definition PublicInput_indDef := [indDef for PublicInput_rect].
-Canonical PublicInput_indType := IndType PublicInput PublicInput_indDef.
-Definition PublicInput_hasDecEq := [derive hasDecEq for PublicInput].
-HB.instance Definition _ := PublicInput_hasDecEq.
-
-Inductive Input := Skip | DiskRead.
-Inductive Output := Idle | Step.
-
-
-Definition Input_indDef := [indDef for Input_rect].
-Canonical Input_indType := IndType Input Input_indDef.
-Definition Input_hasDecEq := [derive hasDecEq for Input].
-HB.instance Definition _ := Input_hasDecEq.
-
-Definition Output_indDef := [indDef for Output_rect].
-Canonical Output_indType := IndType Output Output_indDef.
-Definition Output_hasDecEq := [derive hasDecEq for Output].
-HB.instance Definition _ := Output_hasDecEq.
-
-Inductive Ty : Set := Nat | Times : Ty -> Ty -> Ty | Bool
-                 | Option : Ty -> Ty | Sum : Ty -> Ty -> Ty | TInput | TOutput | TTypeSyscall | Unit | Unit1 | Unit2 |  TInterrupt | THandlerOutput |  TPublicOutput | TPublicInput. 
-
-Derive NoConfusion for Ty.
-Derive EqDec for Ty.
-
-Definition Ty_indDef := [indDef for Ty_rect].
-Canonical Ty_indType := IndType Ty Ty_indDef.
-Definition Ty_hasDecEq := [derive hasDecEq for Ty].
-HB.instance Definition _ := Ty_hasDecEq.
-
-Fixpoint interp (t : Ty) : Set :=
-  match t with
-  | Nat => nat
-  | Times t0 t1 => (interp t0) * (interp t1)
-  | Bool => bool
-  | Option t' => option (interp t')
-  | TInput => Input
-  | TOutput => Output
-  | Sum t0 t1 => (interp t0) + (interp t1)            
-  | TTypeSyscall => TypeSyscall
-  | Unit | Unit1 | Unit2 => unit                     
-  | TInterrupt => Interrupt
-  | THandlerOutput => HandlerOutput
-  | TPublicOutput => PublicOutput
-  | TPublicInput => PublicInput                       
-  end.
-Notation "[ i ]" := (interp i).
-
-
-
-(*Record Inv (I I' : Ty) := mkInv {
-  inv_fn :> [I] -> [I'];
-  inv_pf : forall o : [I'], exists i : [I], inv_fn i = o
-}.*)
-
-(** Process type **)
-Inductive Proc : Ty -> Ty -> Type :=
-| out  : forall {I O : Ty}, interp O -> Proc I O  
-| map   : forall {I I' O O' : Ty}, (interp I -> interp I') -> (interp O -> interp O') -> Proc I' O -> Proc I O'
-| sta   : forall {I O V :Ty}, (interp I -> interp V -> interp V) -> (interp O -> interp V -> interp V) -> interp V -> Proc (Times V I) O -> Proc I (Times V O)
-| swi   : forall {I O : Ty},  bool -> Proc I (Times Bool O)%type -> Proc ((Times Bool I)) (Option O)
-| par   : forall {I O1 O2: Ty}, Proc I O1 -> Proc I O2 -> Proc I (Times O1 O2)
-| loop  : forall {I : Ty}, Proc I I -> Proc I I
-| maybe : forall {I O: Ty}, Proc I O -> Proc (Option I) O.
-Arguments out {_} {_} o.
-Derive NoConfusion for Proc.
-Derive NoConfusionHom for Proc.
-Derive Signature for Proc.
-
-Definition xor (b1 b2 : bool) := (Datatypes.negb (b1 == b2)).
-
-Lemma xorK : forall x y, xor (xor x y) y = x.
-Proof. by destruct x, y. Qed.
-
-Lemma xorC : forall x y, xor x y = xor y x.
-Proof. by destruct x, y. Qed.
-
-Lemma xorFalse : forall x, xor x false = x.
-Proof. by destruct x. Qed.
-
-Lemma xorTrue : forall x, xor x true = negb x.
-Proof. by destruct x. Qed.
-
-Inductive reduceI : forall (I O : Ty), Proc I O -> interp I -> Proc I O -> Prop :=
-| reduce_outI I O i (o : [O]) : reduceI ( @out I _ o) i ( @out I _ o)
-| reduce_mapI (I I' O O' : Ty) p p' i i' (f : [I] -> [I']) (g : [O] -> [O']) : f i = i' -> reduceI p i' p' -> reduceI (map f g p) i (map f g p')
-| reduce_staI (V I O : Ty) v v' (p : Proc (Times V I) O) p' i (f : [I] -> [V] -> [V]) (g : [O] -> [V] -> [V]) : f i v = v' -> reduceI p (v', i) p' -> reduceI (sta f g v p) i (sta f g v' p')
-| reduce_swiI (I O : Ty) b b' b'' (p : Proc I (Times Bool O)) p' (i : [I]) : b'' = xor b b' -> reduceI p i p' -> reduceI (swi b p) (b', i) (swi b'' p')
-| reduce_maybeI (I O : Ty) (p : Proc I O) : reduceI (maybe p) None (maybe p)
-| reduce_maybeI2 (I O : Ty) (p p' : Proc I O) (i : [I]) : reduceI p i p' -> reduceI (maybe p) (Some i) (maybe p')
-| reduce_parI (I O1 O2 : Ty) (p1 p1' : Proc I O1) (p2 p2' : Proc I O2) (i : [I]) : reduceI p1 i p1' -> reduceI p2 i p2' -> reduceI (par p1 p2) i (par p1' p2')
-| reduce_loopI (I :Ty) (p p' : Proc I I) (i : [I]) : reduceI p i p' -> reduceI (loop p) i (loop p').
-
-Hint Constructors reduceI : core.
-
-(*Create HintDb omitdb.
-Hint Resolve reduce_mapI reduce_staI reduce_swiI reduce_maybeI reduce_maybeI2 reduce_parI reduce_loopI : omitdb.*)
-
-Inductive reduceO : forall (I O : Ty), Proc I O -> [O] -> Proc I O -> Prop :=
-| reduce_outO (I O : Ty) (o : [O]) : reduceO ( @out I _ o) o ( @out I _ o)
-| reduce_mapO (I I' O O' : Ty) p p' o o' (f : [I] -> [I']) (g : [O] ->  [O']) : g o = o' -> reduceO p o p' -> reduceO (map f g p) o' (map f g p')
-| reduce_staO (V I O : Ty) v v' p p' o (f : [I] -> [V] -> [V]) (g : [O] -> [V] -> [V]) : g o v = v' -> reduceO p o p' -> reduceO (sta f g v p) (v', o) (sta f g v' p')
-| reduce_swiO (I O : Ty) (p : Proc I (Times Bool O)): reduceO (swi false p) None (swi false p)
-| reduce_swiO2 (I O : Ty) b b' (p : Proc I (Times Bool O)) p' (o : [O]) : b' = xor true b -> reduceO p (b, o) p' -> reduceO (swi true p) (Some o) (swi b' p')
-| reduce_maybeO (I O : Ty) (p p' : Proc I O) (o : [O]) : reduceO p o p' -> reduceO (maybe p) o (maybe p')
-| reduce_parO (I O1 O2 : Ty) (p1 p1' : Proc I O1) (p2 p2' : Proc I O2) (o : [O1]) (o' : [O2]) : reduceO p1 o p1' -> reduceO p2 o' p2' -> reduceO (par p1 p2) (o, o') (par p1' p2')
-| reduce_loopO (O :Ty) (p p' p'' : Proc O O) (o : [O]) : reduceO p o p' -> reduceI p' o p'' -> reduceO (loop p) o (loop p'').
-Hint Constructors reduceO : core.
-
-Ltac check_if_var x :=
-  first [ is_var x;fail 1 "Term" x "is not a bare variable" | idtac ].
-
-Ltac match_dd_once := 
-    match goal with
-    | H : reduceI ?p _ _ |- _ => check_if_var p; dependent destruction  H
-    | H : reduceO ?p _ _ |- _ => check_if_var p; dependent destruction  H
-    end.
-
-
-Ltac match_dd := 
-   repeat match_dd_once.
-
-Ltac match_dd_o := 
-   repeat (match_dd_once;eauto).
-
-
-Inductive Trace (I O : Ty) (ORel : myrel [O]) (l : level) : list ([I] + [O]) -> Proc I O -> Prop :=
-| TR0 p : Trace ORel l nil p
-| TR1 p i p' t : reduceI p i p' -> Trace ORel l t p' -> Trace ORel l (inl i::t) p
-| TR2 p o' o p' t : reduceO p o' p' -> rel ORel l o' o -> Trace ORel l t p' -> Trace ORel l (inr o::t) p.
-Hint Constructors Trace.
-
-Fixpoint insert (A : Set) (n : nat) (a : A) (l : seq A) :=
+Fixpoint sum_N n (f : nat -> Ty) : Ty :=
+  let t := f n in
   match n with
-  | 0 => a::l
-  | n'.+1 => if l is a'::l' then a'::(insert n' a l') else nil
+  | 0 => t
+  | S n' => Sum t (sum_N n' f)
   end.
 
-Fixpoint remove (A : Set) (n : nat) (l : seq A) :=
+Fixpoint times_N n (f : nat -> Ty) : Ty :=
+  let t := f n in
   match n with
-  | 0 => if l is a::l' then l' else nil
-  | n'.+1 => if l is a::l' then a::(remove n' l') else nil
+  | 0 => t
+  | S n' => Times t (times_N n' f)
   end.
 
-Definition NI_l (I O : Ty) (IRel : myrel [I]) (ORel : myrel [O]) (l : level) (p : Proc I O) : Prop :=
-  (forall t i i' n, rel IRel l i i' -> Trace ORel l (insert n (inl i) t) p -> Trace ORel l (insert n (inl i') t) p) /\
-  (forall t i n, dis IRel l i -> Trace ORel l t p -> Trace ORel l (insert n (inl i) t) p) /\
-  (forall t i n, dis IRel l i -> Trace ORel l (insert n (inl i) t) p -> Trace ORel l t p).
+Definition map_option (A B : Set) (f : A -> B) (x : option A) : option B := if x is Some x' then Some (f x') else None.
+Definition map_sum {A B C D :Set} (f : A -> C) (g : B -> D) := fun (x: A + B) => match x with
+                                                                                | inl x' => inl (f x')
+                                                                                | inr x' => inr (g x')
+                                                                                 end.
+Definition map_pair {A B C D :Set} (f : A -> C) (g : B -> D) := fun (x: A * B) => match x with
+                                                                                | (x0,x1) => (f x0, g x1)
+                                                                                  end.
+Definition times_Option_n (n : nat) (f : nat -> Ty) := times_N n (Option \o f).
+
+(*Example*)
+Definition my_f_I := fun (n : nat) => match n with
+                                      | 0 => TInterrupt (*handler*)
+                                      | 1 => THandlerOutput (*private*)
+                                      | 2 => Unit (*public*)
+                                      | 3 => Sum TInterrupt THandlerOutput (*scheduler*)
+                                      | _ => Unit
+                                      end.
+
+Definition my_f_O := fun (n : nat) => match n with
+                                      | 0 => THandlerOutput
+                                      | 1 => TTypeSyscall
+                                      | 2 => TPublicOutput
+                                      | 3 => Times Nat Nat
+                                      | _ => Unit
+                                      end.
+Definition my_T_in := Sum Unit TInterrupt. (*We need Unit input to be able to differentiate trace, otherwise we only have interrupts in the trace*)
+Definition my_T_out := Option (Sum TPublicOutput TTypeSyscall).
+Definition my_T_in' := Times (Times Nat Nat) (times_Option_n 3 my_f_I).
+Definition my_T_out' := times_Option_n 3 my_f_O.
 
 
-Definition NI (I O : Ty) (IRel : myrel [I]) (ORel : myrel [O]) (p : Proc I O) := forall l, NI_l IRel ORel l p.
+(*Process*)
 
+Definition alternate_generic (A B C: Ty) (x y : [B]) (z : [C]) := @map _ (Sum _ _) (Sum _ (Times Bool C)) B 
+                        inl
+                        (fun o => if o is inr (true,z) then x else y)
+                        (@loop (Sum A (Times Bool C))
+                        (@map (Sum A _) _ _ (Sum _ _) id (fun o => inr o)
+                        ((@sta (Sum _ _) _ Bool
+                           (fun i v => if i is inl _ then true else false)
+                           (fun o v => v)
+                           false
+                           (@out (Times Bool _ ) C z)
+                        )))).
 
-Definition boolRel : myrel ([Bool]).
-  refine (@MyRel _
-            (fun l (b : [Bool]) => b \/ l = \bot)
-            (fun l b1 b2 => b1 = b2 \/  (b1 \/ l = \bot) /\ (b2 \/ l = \bot))
-            _
-            _
-            _
-            _).
-intros.
-con. intro. intros. auto. intro. intros. de H. intro. intros. de H. subst. de H0. de H0. subst. de H.
-intros. de H0. de H0. de H1. subst.
-rewrite /order in H.
-rewrite lex0 in H. rewrite (eqP H). de a0.
-subst.
-rewrite /order in H.
-rewrite lex0 in H. rewrite (eqP H). de a0.
-intros. de H0. subst.
-rewrite /order in H.
-rewrite lex0 in H. right. apply/eqP. done.
-intros. con. intros. de H. de H.
-de H0. de a0.
+Definition alternate_generic2 (A B C : Ty) (x y : [B]) (z : [C]) (pred : [A] -> bool) :=
+  @map _ (Sum _ _) (Sum _ (Times Bool C)) B 
+                        inl
+                        (fun o => if o is inr (true,z) then x else y)
+                        (@loop (Sum A (Times Bool C))
+                        (@map (Sum A _) _ _ (Sum _ _) id (fun o => inr o)
+                        ((@sta (Sum _ _) _ Bool
+                           (fun i v => match i with | inl i' => v || pred i' | _ => false end)
+                           (fun o v => v)
+                           false
+                           (@out (Times Bool _ ) C z)
+                        )))).
+
+Definition scheduled_process_pool
+  (n : nat)
+  (f_coopt : nat -> bool)
+  (f_initial : nat -> bool)
+  (f_I f_O : nat -> Ty)
+  (f_proc : forall n, Proc (f_I n) (f_O n)) : Proc (Times (Times Nat Nat) ((times_Option_n n f_I))) (times_Option_n n f_O).
+  elim: n.
+  - simpl.
+    eapply map. simpl.
+      instantiate (1:= Times Bool (Option (f_I 0))). exact (fun n => ((0.+1 \in [:: fst (fst n); snd (fst n)],snd n))).
+      exact id. 
+    eapply swi. exact (f_initial 0.+1). 
+    eapply maybe. 
+    eapply map.
+      eapply id. 
+      exact (fun o => (f_coopt 0.+1,o)).
+    exact (f_proc 0).
+
+  - intros. simpl.
+    eapply par.
+    * eapply map.
+      instantiate (1:= Times Bool (Option (f_I n.+1))). simpl.
+      exact (fun x => ((n.+2) \in [:: fst (fst x); snd (fst x)], fst (snd x))).
+        exact id. 
+      eapply swi.
+        exact (f_initial n.+2). 
+      eapply maybe.
+      eapply map.
+        exact id.     
+        exact (fun o => (f_coopt n.+2,o)).
+      (*eapply maybe.*) (*not necessary anymore*)
+      exact (f_proc n.+1).
+    * eapply map. 3: apply H. simpl. 
+      exact (map_pair id snd).
+      exact id. 
 Defined.
 
-Definition falseRel : myrel ([Bool]).
-  refine (@MyRel _
-            (fun l (b : [Bool]) => ~~ b /\ l = \bot)
-            (fun l b1 b2 => b1 = b2)
-            _
-            _
-            _
-            _).
-  intros. done.
-  intros. ssa. subst. rewrite /order in H. rewrite lex0 in H. apply/eqP. done.
-  intros. ssa. con. ssa. subst. de a1. de a0.
-  intros. subst. ssa.
-Defined.
-
-Definition publicRel (A : Ty) : myrel ([A]).
-  refine (@MyRel _
-            (fun l b => False)
-            (fun l b1 b2 => b1 = b2)
-            _
-            _
-            _
-            _).
-intros.
-done.
-eauto.
-eauto.
-intros. done.
-Defined.
-
-Definition toPublicRel (A : Ty) (ARel : myrel [A]) : myrel ([A]).
-  refine (@MyRel _
-            (fun l b => False)
-            (rel ARel)
-            _
-            _
-            _
-            _).
-intros. all: de ARel. eauto.
-Defined.
-
-Lemma order_bot : forall (l : level), order l \bot -> l = \bot.
-Proof.
-intros.
-rewrite /order lex0 in H.
-by apply/eqP.
-Qed.
-
-
-Lemma not_booleq : forall (A : eqType) (a : A), a != a -> False.
-Proof.
-intros.
-move/eqP : H.
-done.
-Qed.
-Hint Resolve not_booleq.
-
-Definition privateRel (A : Ty) : myrel ([A]).
-  refine (@MyRel _
-            (fun l b => True)
-            (fun l b1 b2 => True) (*Since everything is always hidden, there the value space is an equivalence class*)
-            _
-            _
-            _
-            _).
-intros.
-done. done.
-intros. done. done.
-Defined.
-
-  
-Definition semiprivateRel (A : Ty) : myrel ([A]).
-  refine (@MyRel _
-            (fun l b => l = \bot)
-            (fun l b1 b2 => l <> \bot /\ b1 = b2 \/ l = \bot)
-            _
-            _
-            _
-            _).
-  - intros l. con. 
-    + intro. destruct (eqVneq l \bot). auto.  left. split_and. intro. subst. rewrite eqxx in i. done.
-    + intros x y. case. ssa. intros. subst. auto.
-      intro. intros. destruct H. destruct H0. ssa. subst. auto. ssa. ssa.
-      intros. de H0. subst.
-      destruct (eqVneq l0 \bot). auto. left. split_and. intro. subst. rewrite eqxx in i. done.
-      subst. apply order_bot in H. subst. auto.
-      intros. subst. apply order_bot in H. subst. done.
-      intros. subst. con. auto. auto.
-Defined.
-
-
-Definition eqpair {I O : Ty} (IRel : myrel [I]) (ORel : myrel [O]) : myrel ([Times I O]).
-  refine (@MyRel _ 
-            (fun (l : level) _ => False)
-            (fun l io1 io2 => rel IRel l (fst io1) (fst io2) /\ rel ORel l (snd io1) (snd io2))
-            _
-            _
-            _
-            _).
-  - move=> l. 
-    con. destruct IRel. destruct ORel. simpl. con.
-    move: (equiv0 l). case. eauto.
-    move: (equiv1 l). case. eauto.
-  - con. destruct H. destruct IRel. destruct ORel. simpl. 
-    move: (equiv0 l). case.
-    move => _ Hsym _.  apply Hsym. eauto.
-
-    destruct H. destruct IRel. destruct ORel. simpl. 
-    move: (equiv1 l). case. eauto.
-
-  - destruct IRel,ORel. simpl. con.
-    ssa. move: (equiv0 l). case. move=> _ _ Htrans. eauto.
-    ssa. move: (equiv1 l). case. move=> _ _ Htrans. eauto.
-
-
-  - move=> l0 l1 HOrder a0 a1 [] HI HO.
-    destruct IRel,ORel;ssa. eauto. eauto.
-
-  - eauto.
-
-    intros. con.
-done.
-done.
-Defined.
-
-Definition eqpair_LR {I O : Ty} (IRel : myrel [I]) (ORel : myrel [O]) : myrel ([Times I O]).
-  refine (@MyRel _ 
-            (fun (l : level) io => dis IRel l (fst io) /\ dis ORel l (snd io))
-            (fun l io1 io2 => rel IRel l (fst io1) (fst io2) /\ rel ORel l (snd io1) (snd io2))
-            _
-            _
-            _
-            _).
-  - move=> l. 
-    con. destruct IRel. destruct ORel. simpl. con.
-    move: (equiv0 l). case. eauto.
-    move: (equiv1 l). case. eauto.
-  - con. destruct H. destruct IRel. destruct ORel. simpl. 
-    move: (equiv0 l). case.
-    move => _ Hsym _.  apply Hsym. eauto.
-
-    destruct H. destruct IRel. destruct ORel. simpl. 
-    move: (equiv1 l). case. eauto.
-
-  - destruct IRel,ORel. simpl. con.
-    ssa. move: (equiv0 l). case. move=> _ _ Htrans. eauto.
-    ssa. move: (equiv1 l). case. move=> _ _ Htrans. eauto.
-
-
-  - move=> l0 l1 HOrder a0 a1 [] HI HO.
-    destruct IRel,ORel;ssa. eauto. eauto.
-
-  - intros. ssa. de IRel. eauto. de ORel. eauto.
-  - intros. ssa. de IRel. con.
-    ssa. apply/i;eauto.
-    de ORel. apply/i0;eauto.
-    ssa. apply/i;eauto.
-    de ORel. apply/i0;eauto.
-Defined.
-
-Definition eqpair_L {I O : Ty} (IRel : myrel [I]) (ORel : myrel [O]) : myrel ([Times I O]).
-  refine (@MyRel _ 
-            (fun (l : level) io => dis IRel l (fst io))
-            (fun l io1 io2 => rel IRel l (fst io1) (fst io2) /\ rel ORel l (snd io1) (snd io2) \/ dis IRel l (fst io1) /\ dis IRel l (fst io2))
-            _
-            _
-            _
-            _).
-  - move=> l. 
-    con. destruct IRel. destruct ORel. simpl. con.
-    move: (equiv0 l). case. eauto.
-    move: (equiv1 l). case. eauto.
-  - rewrite /Symmetric. intros. destruct H. destruct IRel. destruct ORel. simpl.
-    ssa. left.
-    move: (equiv0 l). case.
-    move => _ Hsym _. con.  apply Hsym. eauto.
-
-    move: (equiv1 l). case.
-    move => _ Hsym' _.  apply Hsym'. eauto.
-
-    ssa.
-
-  - destruct IRel,ORel. simpl. intro. intros.
-
-    de H. de H0. left. ssa.
-    move: (equiv0 l). case. move=> _ _ Htrans. eauto.
-    move: (equiv1 l). case. move=> _ _ Htrans. eauto.
-
-    right. ssa. apply/i. apply: H0.
-    move: (equiv0 l). case.
-    move=> _ Hsym _. apply/Hsym. done.
-
-    de H0.
-
-    right. ssa. apply/i. apply: H1. done.
-
-
-  - intros. de H0.
-    left.
-    de IRel;eauto.
-    de ORel;eauto.
-    right.
-    de IRel;eauto.
-
-  - intros. de IRel;eauto.
-
-  - intros. con.
-    intros. eauto.
-    case. case. move=> HH _.
-    de IRel;eauto. apply/i. 2:eauto. done.
-    ssa.
-Defined.
-
-Definition eqpair_R {I O : Ty} (IRel : myrel [I]) (ORel : myrel [O]) : myrel ([Times I O]).
-  refine (@MyRel _ 
-            (fun (l : level) io => dis ORel l (snd io))
-            (fun l io1 io2 => rel IRel l (fst io1) (fst io2) /\ rel ORel l (snd io1) (snd io2) \/ dis ORel l (snd io1) /\ dis ORel l (snd io2))
-            _
-            _
-            _
-            _).
-  - move=> l. 
-    con. destruct IRel. destruct ORel. simpl. con.
-    move: (equiv0 l). case. eauto.
-    move: (equiv1 l). case. eauto.
-  - rewrite /Symmetric. intros. destruct H. destruct IRel. destruct ORel. simpl.
-    ssa. left.
-    move: (equiv0 l). case.
-    move => _ Hsym _. con.  apply Hsym. eauto.
-
-    move: (equiv1 l). case.
-    move => _ Hsym' _.  apply Hsym'. eauto.
-
-    ssa.
-
-  - destruct IRel,ORel. simpl. intro. intros.
-
-    de H. de H0. left. ssa.
-    move: (equiv0 l). case. move=> _ _ Htrans. eauto.
-    move: (equiv1 l). case. move=> _ _ Htrans. eauto.
-
-    right. ssa. apply/i0. apply: H0.
-    move: (equiv1 l). case.
-    move=> _ Hsym _. apply/Hsym. done.
-
-    de H0.
-
-    right. ssa. apply/i0. apply: H1. done.
-
-
-  - intros. de H0.
-    left.
-    de IRel;eauto.
-    de ORel;eauto.
-    right.
-    de IRel;eauto.
-
-  - intros. de ORel;eauto. de ORel;eauto.
-
-  - intros. de ORel;eauto.
-    intros. con. ssa.
-    case. case. intros. de ORel. apply/i. 2:eauto. done.
-    case. ssa.
-Defined.
-
-Definition eqpair_REQ {I O : Ty} (def : [I]) (ORel : myrel [O]) : myrel ([Times I O]).
-  refine (@MyRel _ 
-            (fun (l : level) io => fst io = def /\ dis ORel l (snd io))
-            (fun l io1 io2 => rel (publicRel _) l (fst io1) (fst io2) /\ rel ORel l (snd io1) (snd io2) \/ fst io1 = fst io2 /\ dis ORel l (snd io1) /\ dis ORel l (snd io2))
-            _
-            _
-            _
-            _).
-  - move=> l. 
-    con.  destruct ORel. simpl. con.
-    move: (equiv0 l). case. eauto.
-  - rewrite /Symmetric. intros. destruct H. destruct ORel. simpl.
-    ssa. left.
-    move: (equiv0 l). case.
-    move => _ Hsym _. con.  symmetry. done.
-    eauto.
-    ssa. 
-
-  - destruct ORel. simpl. intro. intros.
-
-    de H. de H0. left. ssa.
-    move: (equiv0 l). case. move=> _ _ Htrans. rewrite H H0. done.
-    move: (equiv0 l). case. move=> Hrefl0 _ Htrans0. eauto.
-    move: (equiv0 l). case. move=> Hrefl0 _ Htrans0. eauto.    
-    left. con. rewrite H H0. done. apply/Htrans0. eauto.
-    apply i. done. done.
-    destruct H0. ssa. left. con.
-    move: (equiv0 l). case. move=> Hrefl _ Htrans. by rewrite H H0.
-
-    move: (equiv0 l). case. move=> Hrefl0 _ Htrans0. 
-    apply/Htrans0. 2:eauto.
-    apply i. done. done. ssa.
-    rewrite H H0. ssa.
-
-  - intros. de H0.
-    left. ssa.
-    de ORel;eauto. 
-    left. ssa. de ORel. eapply r.
-     eauto. apply i. done. done.
-  - intros. de ORel;eauto. de ORel;eauto.
-
-  - intros. 
-    intros. con. ssa. left. ssa. rewrite H -H1. done. apply i. done. done.
-    ssa. destruct H1. ssa. rewrite -H1 H. done. ssa. rewrite -H1 H. done.
-    destruct H1. ssa. apply/i. 2:eauto. done.
-    ssa.
-Defined.
-
-Lemma dis_rel_dis : forall (I : Ty) (IRel : myrel [I]) l x y, dis IRel l x -> rel IRel l x y -> dis IRel l y.
-Proof.
-  intros. de IRel. apply/i;eauto.
-Qed.
-Lemma dis_rel_dis2 : forall (I : Ty) (IRel : myrel [I]) l x y, dis IRel l x -> rel IRel l y x -> dis IRel l y.
-Proof.
-  intros. de IRel. apply/i;eauto.
-  move:(equiv0 l)=> [] _ Hsym _. apply/Hsym. auto.
-Qed.
-Lemma dis_dis_rel : forall (I : Ty) (IRel : myrel [I]) l x y, dis IRel l x -> dis IRel l y -> rel IRel l x y.
-Proof.
-  intros. de IRel;eauto. apply/i;eauto.
-Qed.
-
-
-Hint Resolve dis_rel_dis dis_rel_dis2 dis_dis_rel.
-
-
-
-Definition eqpair_OR {I O : Ty} (IRel : myrel [I]) (ORel : myrel [O]) : myrel ([Times I O]).
-  refine (@MyRel _ 
-            (fun (l : level) io => dis IRel l (fst io) \/ dis ORel l (snd io))
-            (fun l io1 io2 => rel IRel l (fst io1) (fst io2) /\ rel ORel l (snd io1) (snd io2) \/
-                                (dis IRel l (fst io1) \/ dis ORel l (snd io1)) /\
-                                (dis IRel l (fst io2) \/ dis ORel l (snd io2))                                  
-            )
-            _
-            _
-            _
-            _).
-  - move=> l. 
-    con. destruct IRel. destruct ORel. simpl. con.
-    move: (equiv0 l). case. eauto.
-    move: (equiv1 l). case. eauto.
-  - intro. intros. destruct H.
-    left. destruct IRel,ORel. simpl in *.
-    destruct H.
-    con.
-    move: (equiv0 l)=> [] _ Hsym _.
-    apply/Hsym. done.
-    move: (equiv1 l)=> [] _ Hsym _.
-    apply/Hsym. done. ssa.
-
-    
-    intro. intros.
-    de H.
-    * de H0.
-      ** left. con.
-         de IRel. move: (equiv0 l)=>[] _ _ Htrans. apply/Htrans;eauto.
-         de ORel. move: (equiv0 l)=>[] _ _ Htrans. apply/Htrans;eauto.    
-      ** de H0. have: dis IRel l x.1 by eauto. move=>HH.
-         right. con. auto. auto.
-         have: dis ORel l x.2 by eauto. move=>HH.
-         right. con. auto. auto.
-    * de H0. right. con. auto.
-      de H1. eauto. eauto.
-
-
-      intros. destruct H0.
-      ** left. destruct IRel. destruct ORel. simpl in *. ssa;eauto.
-      ** right. destruct IRel. destruct ORel. simpl in *. ssa;eauto.
-         de H0;eauto. de H1;eauto.
-
-
-         intros. destruct IRel. destruct ORel. simpl in *.
-         destruct H0;eauto.
-
-
-         intros. con. intros. de H.
-         case. case. intros. de H. eauto. eauto.
-         de H.
-Defined.
-
-Lemma eqsum_LR {I O : Ty} (IRel : myrel [I]) (ORel : myrel [O]) : myrel ([Sum I O]).
-  refine (@MyRel _ 
-            (fun (l : level) io => match io with | inl i => dis IRel l i | inr o => dis ORel l o end)
-            (fun l io1 io2 => match io1,io2 with | inl i1,inl i2 => rel IRel l i1 i2
-                                            | inr o1,inr o2 => rel ORel l o1 o2
-                                            | inl i1, inr i2 => dis IRel l i1 /\ dis ORel l i2
-                                            | inr i1, inl i2 => dis ORel l i1 /\ dis IRel l i2 end)
-            _
-            _
-            _
-            _).
-  - move=> l. 
-    con.
-    intro. 
-    destruct IRel. destruct ORel. simpl. de x.
-    move: (equiv0 l). case. eauto.
-    move: (equiv1 l). case. eauto.
-
-    destruct IRel. destruct ORel. simpl.
-    intro. ssa. de x. de y.
-    move: (equiv0 l). case. eauto. 
-    move: (equiv1 l). case. de y.
-
-    destruct IRel. destruct ORel. simpl.
-    intro. ssa. de x. de y. de z.
-    move: (equiv0 l). case. eauto. apply/i. 2:eauto.
-    move: (equiv1 l). case. eauto.
-
-    move: (equiv0 l). case. eauto. 
-    de z. apply/i. done. done.
-    apply/i0. eauto.
-    done.
-    de y. de z. apply/i. 2:eauto. done.
-    apply/i0. done. done.
-    de z. apply/i0. eauto.
-    move:(equiv1 l)=> [] _ Hsym _. eauto.
-    move:(equiv1 l)=> [] _ _ Htrans. eauto.
-
-
-    intros. de a0. de a1. de IRel;eauto. de IRel;eauto.
-    de ORel;eauto.
-    de a1. de ORel;eauto. de IRel;eauto. de ORel;eauto.
-
-
-    intros. de a. de IRel;eauto. de ORel;eauto.
-
-    intros. con.
-    intros. de a0. de a1. de a1.
-    de a0. de a1. eauto.
-    de a1. eauto.
-Defined.
-
-Lemma eqsum_L {I O : Ty} (IRel : myrel [I]) (ORel : myrel [O]) : myrel ([Sum I O]).
-  refine (@MyRel _ 
-            (fun (l : level) io => match io with | inl i => dis IRel l i | inr _ => False  end)
-            (fun l io1 io2 => match io1,io2 with | inl i1,inl i2 => rel IRel l i1 i2
-                                            | inr o1,inr o2 => rel ORel l o1 o2
-                                            | _,_ => False end)
-            _
-            _
-            _
-            _).
-  - move=> l. 
-    con.
-    intro. 
-    destruct IRel. destruct ORel. simpl. de x.
-    move: (equiv0 l). case. eauto.
-    move: (equiv1 l). case. eauto.
-
-    destruct IRel. destruct ORel. simpl.
-    intro. ssa. de x. de y.
-    move: (equiv0 l). case. eauto. 
-    move: (equiv1 l). case. de y.
-
-    destruct IRel. destruct ORel. simpl.
-    intro. ssa. de x. de y. de z.
-    move: (equiv0 l). case. eauto. de y. de z. 
-    move: (equiv1 l). case. move=> _ _ Htrans. apply/Htrans. eauto. done.
-    intros. de a0. de a1. de IRel;eauto. de IRel;eauto.
-    de ORel;eauto.
-    de a1. eauto.
-    
-    intros. de a. de IRel;eauto.
-    
-    intros. con.
-    intros. de a0. de a1. de a0.
-    de a1. 
-    de IRel. apply/i1;eauto.
-Defined.
-
-Lemma eqsum_R {I O : Ty} (IRel : myrel [I]) (ORel : myrel [O]) : myrel ([Sum I O]).
-  refine (@MyRel _ 
-            (fun (l : level) io => match io with | inl _ => False | inr o => dis ORel l o end)
-            (fun l io1 io2 => match io1,io2 with | inl i1,inl i2 => rel IRel l i1 i2
-                                            | inr o1,inr o2 => rel ORel l o1 o2
-                                            | _,_ => False end)
-            _
-            _
-            _
-            _).
-  - move=> l. 
-    con.
-    intro. 
-    destruct IRel. destruct ORel. simpl. de x.
-    move: (equiv0 l). case. eauto.
-    move: (equiv1 l). case. eauto.
-
-    destruct IRel. destruct ORel. simpl.
-    intro. ssa. de x. de y.
-    move: (equiv0 l). case. eauto. 
-    move: (equiv1 l). case. de y.
-
-    destruct IRel. destruct ORel. simpl.
-    intro. ssa. de x. de y. de z.
-    move: (equiv0 l). case. eauto. de y. de z. 
-    move: (equiv1 l). case. move=> _ _ Htrans. apply/Htrans. eauto. done.
-    intros. de a0. de a1. de IRel;eauto. de IRel;eauto.
-    de ORel;eauto.
-    de a1. eauto.
-    
-    intros. de a. de IRel;eauto. de ORel;eauto.
-    
-    intros. con.
-    intros. de a0. de a1. de a0.
-    de a1. 
-    de IRel. de ORel. apply/i2;eauto.
-Defined.
-
-
-
-Lemma eqsum {I O : Ty} (IRel : myrel [I]) (ORel : myrel [O]) : myrel ([Sum I O]).
-  refine (@MyRel _ 
-            (fun (l : level) io => False)
-            (fun l io1 io2 => match io1,io2 with | inl i1,inl i2 => rel IRel l i1 i2
-                                            | inr o1,inr o2 => rel ORel l o1 o2
-                                            | _,_ => False
-                                            end)           
-            _
-            _
-            _
-            _).
-  - move=> l. 
-    con.
-    intro. 
-    destruct IRel. destruct ORel. simpl. de x.
-    move: (equiv0 l). case. eauto.
-    move: (equiv1 l). case. eauto.
-
-    destruct IRel. destruct ORel. simpl.
-    intro. ssa. de x. de y.
-    move: (equiv0 l). case. eauto. 
-    move: (equiv1 l). case. de y.
-
-    destruct IRel. destruct ORel. simpl.
-    intro. ssa. de x. de y. de z.
-    move: (equiv0 l). case. eauto.
-    de z. de y. de y.
-    move: (equiv1 l). case. move=> _ _ Htrans. apply/Htrans. eauto. eauto.
-    intros. de a0. de a1. de IRel;eauto. de IRel;eauto.
-    de ORel;eauto.
-    de a1. eauto.
-    done.
-    intros. con. done.
-    de a0.
-Defined.
-
-Definition levelPred := level -> Prop.
-Definition presP (P:levelPred) := forall x0 x1, order x0 x1 -> P x0 -> P x1.
-
-Lemma rel_refl : forall (A : Ty) (ARel : myrel [A]) l x, rel ARel l x x.
-Proof.
-  intros. de ARel. move:(equiv0 l). case. eauto.
-Qed.
-Lemma rel_sym : forall A (ARel : myrel A) l x y, rel ARel l x y -> rel ARel l y x.
-  Proof.
-    intros. destruct ARel;ssa.
-    move: (equiv0 l). case. ssa.
-  Qed.
-
-Lemma rel_trans : forall A (ARel : myrel A) l x y z, rel ARel l x y -> rel ARel l y z -> rel ARel l x z.
-  Proof.
-    intros. destruct ARel;ssa.
-    move: (equiv0 l). case. ssa. eauto.
-  Qed.
-
-Lemma myrel_rule1 : forall (A : Ty) (ARel : myrel [A]) l0 l1, order l0 l1 -> forall a0 a1 : [A], rel ARel l1 a0 a1 -> rel ARel l0 a0 a1.
-Proof. intros. de ARel. eauto.
-Qed.
-
-Lemma myrel_rule2 : forall (A : Ty) (ARel : myrel [A]), forall l0 l1 : level, order l0 l1 -> forall a : [A], dis ARel l1 a -> dis ARel l0 a.
-Proof. intros. de ARel. eauto.
-Qed.
-
-Print myrel.
-
-Lemma myrel_rule3 : forall (A : Ty) (ARel : myrel [A]), forall (l : level) (a0 : [A]), dis ARel l a0 -> forall a1 : [A], dis ARel l a1 <-> rel ARel l a0 a1.
-Proof. intros. de ARel. 
-Qed.
-
-Hint Resolve rel_refl rel_sym rel_trans myrel_rule1 myrel_rule2 myrel_rule3.
-Definition eqmaybe_dis {V : Ty} (P: levelPred) (VRel : myrel [V]) l (v : [Option V]) := if v is Some v' then dis VRel l v' else ~ P l.
-Definition eqmaybe_aux {V : Ty} (P: levelPred) (VRel : myrel [V]) : presP P -> myrel ([Option V]).
-intros.  
-    refine (@MyRel _
-            (fun l v => eqmaybe_dis P VRel l v)
-            (fun l b1 b2 => match b1,b2 with
-                            | Some v1,Some v2 => rel VRel l v1 v2
-                            | None, None => True
-                            | _,_ => (eqmaybe_dis P VRel l b1) /\ (eqmaybe_dis P VRel l b2)
-                            end)
-            _
-            _
-            _
-            _).
-    intros. con.
-    intro. de x.
-    intro. intros. de x. de y.
-    ssa. de y.
-    intro. intros.
-    de x. de y.
-    de z. eauto. eauto. de z. 
-    de y. de z. eauto.
-
-    intros. de a0. de a1. eauto. eauto. eauto.
-    
-    de a1. eauto. eauto.
-
-    intros. de VRel. de a. eauto. eauto.
-
-    intros. con.
-
-    intros. de a0.
-    de a1. de a1.
-    de a0. de a1. eauto. de a1.
-Defined.    
-
-Definition Option_presP : presP (fun _ => True).
-  rewrite /presP. eauto.
-Qed.
-
-Definition aware (V : Ty) (VRel : myrel [V]) (v : [V]) : levelPred
-  := fun l => (forall v', rel VRel l v v' -> v = v' /\ ~ dis VRel l v').
-
-Definition Option_presP_swi (BRel : myrel [Bool]) : presP (fun l => aware BRel true l).
-  rewrite /presP. intros. destruct BRel. move: H0. rewrite /aware. ssa.
-  have: rel0 x0 true v'. eauto. move/H0. ssa.
-  have: rel0 x0 true v'. eauto. move/H0. ssa. eauto.
-Qed.
-
-
-Definition Option_presP_false : presP (fun _ => False).
-  rewrite /presP. eauto.
-Qed.
-
-Definition Option_presP_top : presP (fun l => l <> \bot).
-  rewrite /presP. intros. subst. rewrite /order in H. intro. subst. apply/H0.  rewrite lex0 in H. by apply/eqP.
-Qed.
-
-Definition eqmaybe {V : Ty} (VRel : myrel [V]) : myrel ([Option V]).
-  apply:eqmaybe_aux. apply VRel. apply: Option_presP.
-Defined.
-
-Definition eqmaybe_top {V : Ty} (VRel : myrel [V]) : myrel ([Option V]).
-  apply:eqmaybe_aux. apply VRel. apply: Option_presP_top.
-Defined.
-
-Definition eqmaybe_swi {V : Ty} (VRel : myrel [V]) (BRel : myrel [Bool]) : myrel ([Option V]).
-  apply:eqmaybe_aux. apply VRel. apply: Option_presP_swi. apply BRel.
-Defined. 
-
-Definition eqmaybe_false {V : Ty} (VRel : myrel [V]) : myrel ([Option V]).
-  apply:eqmaybe_aux. apply VRel. apply:Option_presP_false.
-Defined. 
-
-Fixpoint to_rel (ty : Ty): myrel [ty]:=
-      match ty as x return myrel [x] with
-    | TInput => publicRel TInput
-    | THandlerOutput => semiprivateRel THandlerOutput
-    | TTypeSyscall => semiprivateRel TTypeSyscall                                 
-    | TInterrupt => semiprivateRel TInterrupt
-    | Option t => eqmaybe (to_rel t)
-    | Times t0 t1 => eqpair_LR (to_rel t0) (to_rel t1)
-      | Sum t0 t1 => eqsum_LR (to_rel t0) (to_rel t1)
-      | Bool => boolRel
-    | ty' => publicRel ty'
-    end.
-
-Inductive NotSim {I O : Ty} (l : level) (IRel : myrel [I]) (ORel : myrel [O]) : Stream ([I] + [O]) -> Proc I O -> Prop :=
-| NS1 i s p : dis IRel l i -> NotSim l IRel ORel s p -> NotSim l IRel ORel (Cons (inl i) s) p
-| NS2 i s p : dis IRel l i -> (forall p', reduceI p i p' -> NotSim l IRel ORel s p') -> NotSim l IRel ORel s p
-| NS3 i s p : (forall p', (exists i', rel IRel l i i' /\ reduceI p i' p') ->  NotSim l IRel ORel s p') -> NotSim l IRel ORel (Cons (inl i) s) p
-| NS4 o s p : (forall p' o', rel ORel l o o' -> reduceO p o' p' -> NotSim l IRel ORel s p') -> NotSim l IRel ORel (Cons (inr o) s) p.
-    
-Ltac pc := pclearbot.
-Definition streampred (I O : Set) l (IRel : myrel I) (ORel : myrel O) (s : Stream (I + O))  := ForAll (fun x => match x with | Cons (inl x') _ => dis IRel l x' | Cons (inr x') _ => dis ORel l x' end) s.
-
-Lemma rel_eq : forall (I : Set) (IRel : myrel I) (x : I) l, rel IRel l x x.
-Proof.
-  intros. de IRel. ssa.
-  move: (equiv0 l). case. move=> Hr _ _. apply Hr.
-Qed.
-Hint Resolve rel_eq.
-
-
-  Variant ObliviousF {I O : Ty} (ORel : myrel [O]) (l : level) (R : Proc I O -> Prop) : Proc I O -> Prop :=
-  OF1 p : (forall i p', reduceI p i p' -> R p') -> (forall o p', reduceO p o p' -> R p' /\ dis ORel l o) ->  ObliviousF ORel l R p.
-
-Lemma monotone_ObliviousF {I O : Ty} (ORel : myrel [O]) (l : level) : monotone1 (@ObliviousF I O ORel l).
-Proof.
-intro;ssa.
-inv IN;eauto.
-econ;eauto.
-intros.
-move: (H0 _ _ H1). case. eauto.
-Qed.
-Hint Resolve monotone_ObliviousF : paco.
-
-Definition oblivious {I O : Ty} (ORel : myrel [O]) p : levelPred := fun l => paco1 (@ObliviousF I O ORel l) bot1 p.
-
-Definition aware_or_oblivious  {I O : Ty} (ORel : myrel [O]) (o : [O]) (p : Proc I O) : levelPred := fun l => aware ORel o l \/ oblivious ORel p l.
-
-
-Lemma zerol : 0 < 0 = false.
-Proof. done.
-Qed.
-
-Ltac swi_instans :=
-   repeat
-    match goal with
-    | |- context [ swi (?x < ?x) _] => is_evar x; unify x 0; try rewrite zerol
-    | |- context [ swi (?x < ?x != _) _] => is_evar x; unify x 0; try rewrite zerol
-    end; rewrite ?eqxx /= /xor /=.
-
-Ltac reduce_once :=
-  simpl;
-    match goal with
-    | |- reduceI (@out _ _ _) _ _ => apply: reduce_outI
-    | |- reduceI (@map _ _ _ _ _ _ _) _ _ => apply: reduce_mapI
-    | |- reduceI (@sta _ _ _ _ _ _ _) _ _ => apply: reduce_staI
-    | |- reduceI (@swi _ _ _ _) _ _ => apply: reduce_swiI
-    | |- reduceI (par _ _) _ _ => apply: reduce_parI
-    | |- reduceI (@loop _ _) _ _ => apply: reduce_loopI                                                  
-    | |- reduceI (@maybe _ _ _) None _ => apply: reduce_maybeI
-    | |- reduceI (@maybe _ _ _) (Some _) _ => apply: reduce_maybeI2
-
-    | |- reduceO (@out _ _ _) _ _ => apply: reduce_outO
-    | |- reduceO (@map _ _ _ _ _ _ _) _ _ => apply: reduce_mapO
-    | |- reduceO (@sta _ _ _ _ _ _ _) _ _ => apply: reduce_staO
-    | |- reduceO (@swi _ _ _ _) None _ => apply: reduce_swiO
-    | |- reduceO (@swi _ _ _ _) (Some _) _ => apply: reduce_swiO2
-    | |- reduceO (@swi _ _ false _) _ _ => apply: reduce_swiO
-    | |- reduceO (@swi _ _ true _) _ _ => apply: reduce_swiO2                                                       
-    | |- reduceO (par _ _) _ _ => apply: reduce_parO
-    | |- reduceO (@loop _ _) _ _ => apply: reduce_loopO
-    | |- reduceO (@maybe _ _ _) _ _ => apply: reduce_maybeO
-    end.
-
-Ltac debug_reduce :=
-    match goal with
-    | |- reduceI ?p ?i _ => idtac "reduceI" i
-    | |- reduceO ?p ?o _ => idtac "reduceO" o
-    end.
-
-Ltac reduce_once_v :=
-  simpl;
-    match goal with
-    | |- reduceI (@out _ _ _) _ _ => apply: reduce_outI
-    | |- reduceI (@map _ _ _ _ _ _ _) ?i _ => idtac "map_in" i;apply: reduce_mapI
-    | |- reduceI (@sta _ ?O _ _ _ ?v ?p) ?i _ => idtac "state" v;idtac "state input" i;idtac "continuation" p;idtac "output type" O;apply: reduce_staI
-    | |- reduceI (@swi _ _ _ _) _ _ => apply: reduce_swiI
-    | |- reduceI (par _ _) _ _ => apply: reduce_parI
-    | |- reduceI (@loop _ _) _ _ => apply: reduce_loopI                                                  
-    | |- reduceI (@maybe _ _ _) None _ => idtac "maybe none"; apply: reduce_maybeI
-    | |- reduceI (@maybe _ _ _) (Some _) _ => idtac "maybe some"; apply: reduce_maybeI2
-
-    | |- reduceO (@out _ _ _) _ _ => apply: reduce_outO
-    | |- reduceO (@map _ _ _ _ _ _ _) ?o _ => idtac "map_out" o;apply: reduce_mapO
-    | |- reduceO (@sta _ _ _ _ _ ?v _) _ _ => idtac "state" v;apply: reduce_staO
-    | |- reduceO (@swi _ _ _ _) None _ => apply: reduce_swiO
-    | |- reduceO (@swi _ _ _ _) (Some _) _ => apply: reduce_swiO2
-    | |- reduceO (@swi _ _ false _) _ _ => apply: reduce_swiO
-    | |- reduceO (@swi _ _ true _) _ _ => apply: reduce_swiO2                                                       
-    | |- reduceO (par _ _) _ _ => apply: reduce_parO
-    | |- reduceO (@loop _ _) _ _ => apply: reduce_loopO
-    | |- reduceO (@maybe _ _ _) _ _ => apply: reduce_maybeO
-    end.
-
-Ltac controlled_eauto := 
-    match goal with
-    | |- reduceI _ _ _ => idtac
-    | |- reduceO _ _ _ => idtac
-    | |- _ => eauto                        
-    end.
-
-Ltac rewr := idtac. (*updated later*)
-Ltac reduce_tac :=
-  (try rewr);
-   (repeat
-      reduce_once);(try swi_instans);controlled_eauto; rewrite ?eqxx /= /xor /=.
-
-Ltac reduce_tac_v :=
-  (try rewr);(rewrite ?eqxx /= /xor /= );
-   repeat first [reduce_once_v;first try econ | swi_instans].
-
-
-Definition f_NI {I O :Ty} (IRel : myrel [I]) (ORel : myrel [O]) (f : [I] -> [O]) := forall (l : level) (i i' : [I]), rel IRel l i i' -> rel ORel l (f i) (f i').
-Definition f_PU {I O : Ty} (IRel : myrel [I]) (ORel : myrel [O]) (f : [I] -> [O]) := forall l (i : [I]), dis IRel l i -> dis ORel l (f i).
-Definition f_NI_PU {I O : Ty} (IRel : myrel [I]) (ORel : myrel [O]) (f : [I] -> [O])  := f_NI IRel ORel f /\ f_PU IRel ORel f.
-Definition fv_NI (I O V: Ty) (IRel : myrel [I]) (ORel : myrel [O]) (VRel : myrel [V])  (f : [I] -> [V] -> [O]) := forall l (i i' : [I]), rel IRel l i i' -> forall (v v' : [V]), rel VRel l v v' -> rel ORel l (f i v) (f i' v').
-Definition f_EP (I V: Ty) (IRel : myrel [I]) (VRel : myrel [V]) (f : [I] -> [V] -> [V]) := forall l i, dis IRel l i -> forall v, rel VRel l (f i v) v. (*equivalence preserving*)
-
-
- (*fixed typo in paper: In conclusion, replaced I with Bool * I  *)
-Lemma rel_eqpair : forall (A B : Ty) (ARel : myrel [A]) (BRel : myrel [B]) l a b, rel (eqpair ARel BRel) l a b -> rel ARel l a.1 b.1 /\ rel BRel l a.2 b.2.
-Proof.
-  ssa.
-Qed.
-
-Lemma rel_eqpair2 : forall (A B : Ty) (ARel : myrel [A]) (BRel : myrel [B]) l a b, 
-    rel ARel l a.1 b.1 /\ rel BRel l a.2 b.2 -> rel (eqpair ARel BRel) l a b.
-Proof.
-  ssa.
-Qed.
-
-Lemma rel_eqpair_R2 : forall (A B : Ty) (ARel : myrel [A]) (BRel : myrel [B]) l a1 a2 b1 b2,  rel ARel l a1 a2 /\ rel BRel l b1 b2 \/ dis BRel l b1 /\ dis BRel l b2 -> rel (eqpair_R ARel BRel) l (a1,b1) (a2,b2).
-Proof.
-  ssa.
-Qed.
-
-Lemma rel_eqpair_R2' : forall (A B : Ty) (ARel : myrel [A]) (BRel : myrel [B]) l a1 a2 b1 b2, rel (eqpair_R ARel BRel) l (a1,a2) (b1,b2) -> rel ARel l a1 b1 /\ rel BRel l a2 b2  \/ dis BRel l a2 /\ dis BRel l b2.
-Proof.
-  ssa.
-Qed.
-
-Lemma rel_eqpair_L2 : forall (A B : Ty) (ARel : myrel [A]) (BRel : myrel [B]) l a1 a2 b1 b2,  rel ARel l a1 a2 /\ rel BRel l b1 b2 \/ dis ARel l a1 /\ dis ARel l a2 -> rel (eqpair_L ARel BRel) l (a1,b1) (a2,b2).
-Proof.
-  ssa.
-Qed.
-
-Lemma rel_eqpair_L2' : forall (A B : Ty) (ARel : myrel [A]) (BRel : myrel [B]) l a1 a2 b1 b2, rel (eqpair_L ARel BRel) l (a1,b1) (a2,b2) -> rel ARel l a1 a2 /\ rel BRel l b1 b2  \/ dis ARel l a1 /\ dis ARel l a2.
-Proof.
-  ssa.
-Qed.
-
-Lemma rel_eqpair_LR : forall (A B : Ty) (ARel : myrel [A]) (BRel : myrel [B]) l a b, rel (eqpair_LR ARel BRel) l a b -> rel ARel l a.1 b.1 /\ rel BRel l a.2 b.2.
-Proof.
-  ssa.
-Qed.
-
-Lemma rel_eqpair_LR2 : forall (A B : Ty) (ARel : myrel [A]) (BRel : myrel [B]) l a1 a2 b1 b2,  rel ARel l a1 b1 /\ rel BRel l a2 b2 -> rel (eqpair_LR ARel BRel) l (a1,a2) (b1,b2).
-Proof.
-  ssa.
-Qed.
-
-Lemma dis_eqpair_R : forall (A B : Ty) (ARel : myrel [A]) (BRel : myrel [B]) l a b, dis (eqpair_R ARel BRel) l (a,b) -> dis BRel l b.
-Proof.  
-  intros. ssa.
-Qed.
-
-Lemma dis_eqpair_R2 : forall (A B : Ty) (ARel : myrel [A]) (BRel : myrel [B]) l a b, dis BRel l b -> dis (eqpair_R ARel BRel) l (a,b).
-Proof.  
-  intros. ssa.
-Qed.
-
-Lemma dis_eqpair_L : forall (A B : Ty) (ARel : myrel [A]) (BRel : myrel [B]) l a b, dis (eqpair_L ARel BRel) l (a,b) -> dis ARel l a.
-Proof.  
-  intros. ssa.
-Qed.
-
-Lemma dis_eqpair_L2 : forall (A B : Ty) (ARel : myrel [A]) (BRel : myrel [B]) l a b, dis ARel l a -> dis (eqpair_L ARel BRel) l (a,b).
-Proof.  
-  intros. ssa.
-Qed.
-
-Lemma dis_eqpair_LR : forall (A B : Ty) (ARel : myrel [A]) (BRel : myrel [B]) l a b, dis (eqpair_LR ARel BRel) l (a,b) -> dis ARel l a /\ dis BRel l b.
-Proof.  
-  intros. ssa.
-Qed.
-
-Lemma dis_eqpair_LR2 : forall (A B : Ty) (ARel : myrel [A]) (BRel : myrel [B]) l a b, dis ARel l a /\ dis BRel l b -> dis (eqpair_LR ARel BRel) l (a,b).
-Proof.  
-  intros. ssa.
-  Qed.
-
-
-
-
-
-
-
-
-
-
-
-
-Lemma f_NI_id (A : Ty) B : @f_NI A A B B id.
-  rewrite /f_NI. done.
-Qed.
-
-Lemma f_PU_id (A : Ty) B : @f_PU A A B B id.
-  rewrite /f_PU. done.
-Qed.  
-Hint Resolve (*f_NI_eq*) f_NI_id f_PU_id.
-
-Ltac mrw := rewrite /f_NI /f_PU /fv_NI /f_EP.
-
-
-
-
-Lemma f_NI_snd_eqpair : forall (A B : Ty) (ARel : myrel [A]) (BRel : myrel [B]), f_NI (eqpair ARel BRel) BRel snd. 
-Proof.
-mrw. ssa.
-Qed.
-
-Lemma f_NI_snd_eqpair_LR : forall (A B : Ty) (ARel : myrel [A]) (BRel : myrel [B]), f_NI (eqpair_LR ARel BRel) BRel snd. 
-Proof.
-mrw. ssa.
-Qed.
-
-Hint Resolve f_NI_snd_eqpair (*f_NI_snd_eqpair_L f_NI_snd_eqpair_R*) f_NI_snd_eqpair_LR (*f_NI_snd_eqpair_OR*) : tempdb.
-
-Lemma rel_eqsum_LR : forall (A B : Ty) (a1 a2 : [A]) (ARel : myrel [A]) (BRel : myrel [B]) l, rel ARel l a1 a2 -> rel (eqsum_LR ARel BRel) l (inl a1) (inl a2). 
-Proof. ssa.
-Qed.
-
-Lemma rel_eqsum_LR2 : forall (A B : Ty) (b1 b2 : [B]) (ARel : myrel [A]) (BRel : myrel [B]) l, rel BRel l b1 b2 -> rel (eqsum_LR ARel BRel) l (inr b1) (inr b2). 
-Proof. ssa.
-Qed.
-
-Lemma rel_eqsum_LR' : forall (A B : Ty) (a1 a2 : [A]) (ARel : myrel [A]) (BRel : myrel [B]) l,rel (eqsum_LR ARel BRel) l (inl a1) (inl a2) ->  rel ARel l a1 a2. 
-Proof. ssa.
-Qed.
-
-Lemma rel_eqsum_LR2' : forall (A B : Ty) (b1 b2 : [B]) (ARel : myrel [A]) (BRel : myrel [B]) l, rel (eqsum_LR ARel BRel) l (inr b1) (inr b2) -> rel BRel l b1 b2. 
-Proof. ssa.
-Qed.
-
-Lemma dis_eqsum_LR : forall (A B : Ty) (a : [A]) (ARel : myrel [A]) (BRel : myrel [B]) l, dis ARel l a -> dis (eqsum_LR ARel BRel) l (inl a). 
-Proof. ssa.
-Qed.
-
-Lemma dis_eqsum_LR' : forall (A B : Ty) (a : [A]) (ARel : myrel [A]) (BRel : myrel [B]) l,  dis (eqsum_LR ARel BRel) l (inl a) -> dis ARel l a. 
-Proof. ssa.
-Qed.
-
-Lemma rel_eqsum : forall (A B : Ty) (a1 a2 : [A]) (ARel : myrel [A]) (BRel : myrel [B]) l, rel ARel l a1 a2 -> rel (eqsum ARel BRel) l (inl a1) (inl a2). 
-Proof. ssa.
-Qed.
-
-Lemma rel_eqsum2 : forall (A B : Ty) (b1 b2 : [B]) (ARel : myrel [A]) (BRel : myrel [B]) l, rel BRel l b1 b2 -> rel (eqsum ARel BRel) l (inr b1) (inr b2). 
-Proof. ssa.
-Qed.
-
-Lemma rel_eqsum' : forall (A B : Ty) (a1 a2 : [A]) (ARel : myrel [A]) (BRel : myrel [B]) l,rel (eqsum ARel BRel) l (inl a1) (inl a2) ->  rel ARel l a1 a2. 
-Proof. ssa.
-Qed.
-
-Lemma rel_eqsum2' : forall (A B : Ty) (b1 b2 : [B]) (ARel : myrel [A]) (BRel : myrel [B]) l, rel (eqsum ARel BRel) l (inr b1) (inr b2) -> rel BRel l b1 b2. 
-Proof. ssa.
-Qed.
-
-Lemma rel_eqsum_L : forall (A B : Ty) (a1 a2 : [A]) (ARel : myrel [A]) (BRel : myrel [B]) l, rel ARel l a1 a2 -> rel (eqsum_L ARel BRel) l (inl a1) (inl a2). 
-Proof. ssa.
-Qed.
-
-Lemma rel_eqsum_L2 : forall (A B : Ty) (b1 b2 : [B]) (ARel : myrel [A]) (BRel : myrel [B]) l, rel BRel l b1 b2 -> rel (eqsum_L ARel BRel) l (inr b1) (inr b2). 
-Proof. ssa.
-Qed.
-
-Lemma rel_eqsum_L' : forall (A B : Ty) (a1 a2 : [A]) (ARel : myrel [A]) (BRel : myrel [B]) l,rel (eqsum_L ARel BRel) l (inl a1) (inl a2) ->  rel ARel l a1 a2. 
-Proof. ssa.
-Qed.
-
-Lemma rel_eqsum_L2' : forall (A B : Ty) (b1 b2 : [B]) (ARel : myrel [A]) (BRel : myrel [B]) l, rel (eqsum_L ARel BRel) l (inr b1) (inr b2) -> rel BRel l b1 b2. 
-Proof. ssa.
-Qed.
-
-Lemma dis_eqsum_L : forall (A B : Ty) (a : [A]) (ARel : myrel [A]) (BRel : myrel [B]) l, dis ARel l a -> dis (eqsum_L ARel BRel) l (inl a). 
-Proof. ssa.
-Qed.
-
-Lemma dis_eqsum_L2 : forall (A B : Ty) (a : [A]) (ARel : myrel [A]) (BRel : myrel [B]) l, dis (eqsum_L ARel BRel) l (inl a) -> dis ARel l a. 
-Proof. ssa.
-Qed.
-
-Lemma rel_eqsum_R : forall (A B : Ty) (a1 a2 : [A]) (ARel : myrel [A]) (BRel : myrel [B]) l, rel ARel l a1 a2 -> rel (eqsum_R ARel BRel) l (inl a1) (inl a2). 
-Proof. ssa.
-Qed.
-
-Lemma rel_eqsum_R2 : forall (A B : Ty) (b1 b2 : [B]) (ARel : myrel [A]) (BRel : myrel [B]) l, rel BRel l b1 b2 -> rel (eqsum_R ARel BRel) l (inr b1) (inr b2). 
-Proof. ssa.
-Qed.
-
-Lemma rel_eqsum_R' : forall (A B : Ty) (a1 a2 : [A]) (ARel : myrel [A]) (BRel : myrel [B]) l,rel (eqsum_R ARel BRel) l (inl a1) (inl a2) ->  rel ARel l a1 a2. 
-Proof. ssa.
-Qed.
-
-Lemma rel_eqsum_R2' : forall (A B : Ty) (b1 b2 : [B]) (ARel : myrel [A]) (BRel : myrel [B]) l, rel (eqsum_R ARel BRel) l (inr b1) (inr b2) -> rel BRel l b1 b2. 
-Proof. ssa.
-Qed.
-
-Lemma dis_eqsum_R : forall (A B : Ty) (b : [B]) (ARel : myrel [A]) (BRel : myrel [B]) l, dis BRel l b -> dis (eqsum_R ARel BRel) l (inr b). 
-Proof. ssa.
-Qed.
-
-Lemma dis_eqsum_R2 : forall (A B : Ty) (b : [B]) (ARel : myrel [A]) (BRel : myrel [B]) l, dis (eqsum_R ARel BRel) l (inr b) -> dis BRel l b. 
-Proof. ssa.
-Qed.
-
-Lemma rel_eqpair_to_L : forall (A B : Ty) (ARel : myrel [A]) (BRel : myrel [B]) l x y, rel (eqpair ARel BRel) l x y -> rel (eqpair_L ARel BRel) l x y.
-Proof.
-  ssa.
-Qed.
-
-Lemma simp_pair1 : forall (A B: Type) (a : A) (b : B), (a,b).1 = a.
-Proof. done.
-Qed.
-Lemma simp_pair2 : forall (A B: Type) (a : A) (b : B), (a,b).2 = b.
-Proof. done.
-Qed.
-
-Definition pair_rewr := (simp_pair1,simp_pair2).
-
-Lemma rel_eqmaybe : forall (A : Ty) (ARel : myrel [A]) l x y, rel ARel l x y -> rel (eqmaybe ARel) l (Some x) (Some y).
-Proof. ssa.
-Qed.
-
-
-
-
-
-  Lemma rel_eqpair_OR : forall (A B : Ty) (ARel : myrel [A]) (BRel : myrel [B]) l x0 x1 y0 y1,
-      rel (eqpair_OR ARel BRel) l (x0,x1) (y0,y1) -> rel ARel l x0 y0 /\ rel BRel l x1 y1 \/ (dis ARel l x0 \/ dis BRel l x1) /\ (dis ARel l y0 \/ dis BRel l y1).  
-  Proof. ssa.
-  Qed.
-
-  
-  Lemma level_not : forall (l : level), ~ (l <> \bot) -> l = \bot.
-    intros. de (eqVneq l \bot). exfalso. apply H. intro. subst. by rewrite eqxx in i.
-  Qed.
-  Hint Resolve level_not.
-
-
-  Ltac inner_match H := match H with
-                         | context[match ?x with _ => _ end] => first [ inner_match x | idtac x;de x ]
-                         end.                                             
-
-  Ltac temp_tac := (match reverse goal with
-                           | H : _ \/ _ |- _ => de H
-                           | H : match ?x with _ => _ end |- _ => de x
-                           | |- ?H => inner_match H
-                    end                      
-                    ;subst;ssa).
-
-  Lemma rel_eqmaybe_top_aux : forall (A : Ty) (ARel : myrel [A]) l x y, rel (eqmaybe_top ARel) l x y -> match x,y with
-                                                                                              | Some x', Some y' => rel ARel l x' y'
-                                                                                              | Some x', None => l = \bot /\ dis ARel l x'
-                                                                                              | None, Some y' => l = \bot /\ dis ARel l y'
-                                                                                              | None, None => True
-                                                                                                    end.
-  Proof.
-    intros.
-    temp_tac.
-    temp_tac.
-    temp_tac.
-  Qed.
-
-  Lemma rel_eqmaybe_top : forall (A : Ty) (ARel : myrel [A]) l x y, rel (eqmaybe_top ARel) l x y -> (exists x' y', x = Some x' /\ y = Some y' /\ rel ARel l x' y') \/
-                                                                                                      (exists x', x = Some x' /\ y = None /\ l = \bot /\ dis ARel l x') \/
-                                                                                                      (exists y', x = None /\ y = Some y' /\ l = \bot /\ dis ARel l y') \/ x = None /\ y = None.
-  Proof.
-    intros. de x. de y. left. eauto.
-    right. left. econ.  eauto.
-    de y. right. right. econ. econ. eauto.
-  Qed.
-
-  Lemma rel_eqmaybe_top2 : forall (A : Ty) (ARel : myrel [A]) l x y, rel ARel l x y -> rel (eqmaybe_top ARel) l (Some x) (Some y).
-    Proof. ssa.
-    Qed.
-
-  Lemma rel_eqmaybe_false2 : forall (A : Ty) (ARel : myrel [A]) l x y, rel ARel l x y -> rel (eqmaybe_false ARel) l (Some x) (Some y).
-    Proof. ssa.
-    Qed.
-
-    
-  Lemma rel_eqmaybe_aux : forall (A : Ty) (ARel : myrel [A]) l x y, rel (eqmaybe ARel) l x y -> match x,y with
-                                                                                              | Some x', Some y' => rel ARel l x' y'
-                                                                                              | Some x', None => dis ARel l x'
-                                                                                              | None, Some y' => dis ARel l y'
-                                                                                              | None, None => True
-                                                                                                    end.
-  Proof.
-    intros.
-    temp_tac.
-    temp_tac.
-    temp_tac.
-  Qed.
-
-  Lemma rel_eqmaybe2 : forall (A : Ty) (ARel : myrel [A]) l x y, rel (eqmaybe ARel) l x y -> (exists x' y', x = Some x' /\ y = Some y' /\ rel ARel l x' y') \/
-                                                                                               x = None /\ y = None.
-  Proof.
-    intros.
-    de x. de y.
-    left. eauto.
-    de y.
-  Qed.
-
-  Lemma rel_eqmaybe_swi2 : forall (A : Ty) (ARel : myrel [A]) (BRel : myrel [Bool]) l x y, rel (eqmaybe_swi ARel BRel) l x y -> (exists x' y', x = Some x' /\ y = Some y' /\ rel ARel l x' y') \/
-                                                                                               (x = None /\ y = None) \/ (eqmaybe_dis (aware BRel true) ARel l x /\ eqmaybe_dis (aware BRel true) ARel l y).
-  Proof.
-    intros.
-    de x. de y.
-    left. eauto.
-    de y.
-  Qed.
-
-  Lemma dis_eqmaybe : forall (A : Ty) (ARel : myrel [A]) l v, dis (eqmaybe ARel) l v -> exists v', v = Some v' /\ dis ARel l v'.
-  Proof.
-    intros. ssa. de v. econ. eauto.
-  Qed.
-
-  Lemma dis_eqmaybe2 : forall (A : Ty) (ARel : myrel [A]) l x, dis ARel l x -> dis (eqmaybe ARel) l (Some x). 
-  Proof.
-    intros. ssa. 
-  Qed.
-
-  Lemma dis_eqmaybe_false2 : forall (A : Ty) (ARel : myrel [A]) l x, dis ARel l x -> dis (eqmaybe_false ARel) l (Some x). 
-  Proof.
-    intros. ssa. 
-  Qed.    
-
-  Definition is_inl (A B : Set) (x : A + B) := if x is inl _ then true else false.
-  Definition is_inr (A B : Set) (x : A + B) := if x is inr _ then true else false.
-
-  Lemma dis_eqsum_LR2 : forall (A B : Ty) (ARel : myrel [A]) (BRel : myrel [B]) l b, dis BRel l b -> dis (eqsum_LR ARel BRel) l (inr b).
-  Proof. intros. ssa.
-  Qed.
-    
-  Lemma aware_public : aware (publicRel Bool) true \bot.
-  Proof. rewrite /aware. ssa.
-  Qed.
-  Hint Resolve aware_public.
+Definition inr_or_def {A B : Set} (def: B) (x : A + B) := if x is inr x' then x' else def.
+
+Definition only_loop
+  (T_in' T_out' : Ty)   
+  (f_route : [T_out'] -> [T_in'])
+  (def : [T_out'])
+  (p : Proc T_in' T_out')
+  : Proc T_in' T_out' :=
+  (@map T_in' (Sum T_in' T_out') (Sum T_in' T_out') T_out' inl (inr_or_def def)
+                          (@loop (Sum T_in' T_out')
+                             (@map (Sum T_in' T_out')
+                                    T_in'
+                                    _
+                                    (Sum _ _)
+                                (fun i  =>
+                                   match i with
+                                   | inl i' => i'
+                                   | inr o  => f_route o (*i tilfælde hvor vi både ændrer switch og rerouter input, problem?*)
+                                   end) inr
+                                p))).
+
+Definition low_p := @out Unit TPublicOutput GetRequest.
+Definition handler := @alternate_generic TInterrupt THandlerOutput Unit2 Notify Nothing tt.
+Definition high_p := @alternate_generic2 THandlerOutput TTypeSyscall Unit1 Syscall NOP tt (fun i => i == Notify).
 
 (*
-(* ============================================================== *)
-(* NEW APPROACH: one state-threaded list, two projections.        *)
-(*                                                                *)
-(* An element of the threaded list carries the state on whichever *)
-(* side needs it:                                                 *)
-(*   inl (w,i) : an input step  -- w is the post-input state      *)
-(*               (= f i v), i the input.                          *)
-(*   inr (w,o) : an output step -- w is the post-output state     *)
-(*               (= g o v), o the (observed) output.              *)
-(*                                                                *)
-(*   projI drops the state from INPUTS  -> the sta-trace          *)
-(*         (over [I] + [Times V O]).                              *)
-(*   projO drops the state from OUTPUTS -> the p-trace            *)
-(*         (over [Times V I] + [O]).                              *)
-(* ============================================================== *)
+From:
 
-Definition projI (V I O : Ty) (x : [Times V I] + [Times V O]) : [I] + [Times V O] :=
+private on ->(?timerinterrupt)
+private on, scheduler on ->(!(handler_index,private_out))
+handler on ->(!handler_out)
+scheduler on ->(!public_index)
+public on ->(?timerinterrupt)
+public on, scheduler on ->(!(handler_index,public_out))
+handler on ->(!handler_out)
+scheduler on ->(!private_index)
+...
+
+
+To:
+
+private on ->(?timerinterrupt)
+private on ->(!private_out)
+scheduler on ->(!handler_index)
+handler on ->(!handler_out)
+scheduler on ->(!public_index)
+public on ->(?timerinterrupt)
+public on ->(!public_out)
+scheduler on ->(!handler_index)
+handler on ->(!handler_out)
+scheduler on ->(!private_index)
+...
+ *)
+Definition good_schedulerp :  Proc (Sum TInterrupt THandlerOutput) (Times Nat Nat). (*handlerflag, processflag*) Check sta_NI. Check swi_NI. 
+  eapply map. apply id. instantiate (1:= Times (Times Bool Bool) Unit).
+  exact (fun o => match fst o with | (true,false) => (3,1) | (true,true) => (2,1) | (false,true) => (3,3) | (false,false) => (2,2) end ).
+  eapply (@sta _ _ _). exact (fun ih bb => match ih with | inl TimerInterrupt => (true,~~ (snd bb))
+                                                         | inr _ => (false,snd bb)
+                                                         | _ => bb          
+                                           end).
+  exact (fun _ bb => bb).
+  exact (false,false).
+  eapply out. con.
+Defined.
+
+Definition sstream := Stream ([(Sum TInterrupt THandlerOutput)] + [(Times Nat Nat)]).
+
+Definition my_sstreamF (s : sstream) := Cons (inl (inl TimerInterrupt)) (Cons (inr (2,1)) (Cons (inl (inr Nothing)) (Cons (inr (3,3))
+                                                                                                                      (Cons (inl (inl TimerInterrupt)) (Cons (inr (3,1)) (Cons (inl (inr Nothing)) (Cons (inr (2,2)) s))))))).
+
+CoFixpoint my_sstream := my_sstreamF my_sstream.
+
+Lemma my_sstream_eq : my_sstream = my_sstreamF my_sstream.
+Proof.
+rewrite {1}/my_sstream.
+rewrite {1}(coseq_match (cofix my_sstream : sstream := my_sstreamF my_sstream)).
+simpl.
+rewrite /my_sstreamF.
+do ? f_equal.
+Qed.
+
+Lemma schedulerp_trace : trace my_sstream good_schedulerp.
+Proof.
+  pcofix CIH.
+  rewrite my_sstream_eq /my_sstreamF /good_schedulerp.
+  bundle;left.
+  bundle;left.
+  bundle;left.
+  bundle;left.
+  bundle;left.
+  bundle;left.
+  bundle;left.
+  bundle;right.
+Qed.
+
+
+Definition unit_p : Proc Unit Unit := @out Unit Unit tt.
+
+Definition my_procs_good : forall n, Proc (my_f_I n) (my_f_O n).
+  case. apply handler.
+  case. apply high_p.
+  case. apply low_p.
+  case. simpl. apply good_schedulerp.
+  elim. apply unit_p.
+  intros. apply unit_p.
+Defined.
+
+
+
+Definition my_f_coopt n := n == 4.
+Definition my_f_initial n := n == 2.
+Definition process_pool_good := @scheduled_process_pool 3 my_f_coopt my_f_initial my_f_I my_f_O my_procs_good.
+
+
+Definition LoopType_n (n : nat) (f_I f_O : nat -> Ty) := Sum (times_Option_n n f_I) (times_Option_n n f_O).
+Definition None_N (n : nat) (f_O : nat -> Ty) : [(times_Option_n n f_O)].
+elim: n. simpl. exact None.
+intros. simpl. eapply pair. exact None. exact H.
+Defined.
+Definition collapse_in_out (n : nat) (f_I f_O : nat -> Ty) (x : [LoopType_n n f_I f_O]) : [times_Option_n n f_O]  :=
   match x with
-  | inl vi => inl (snd vi)
-  | inr vo => inr vo
+  | inl _ => None_N n f_O
+  | inr x' => x'
   end.
-
-Definition projO (V I O : Ty) (x : [Times V I] + [Times V O]) : [Times V I] + [O] :=
-  match x with
-  | inl vi => inl vi
-  | inr vo => inr (snd vo)
-  end.
-
-(* list-level projections (avoid the name clash with the Proc constructor map) *)
-Fixpoint projIl (V I O : Ty) (t : seq ([Times V I] + [Times V O])) : seq ([I] + [Times V O]) :=
+Definition my_def := None_N 3 my_f_O.
+Definition none4 : [ (times_Option_n 3 my_f_I) ]  := (None,(None,(None,None))).
+Definition my_f_route_good (t : [my_T_out']) : [my_T_in'] :=
   match t with
-  | nil => nil
-  | x :: t' => projI x :: projIl t'
+  | (Some sch,_) => (sch,none4)
+  | (_ ,(Some publ, _)) => ((0,0),none4)
+  | (_ ,(None,(Some prv,_))) => ((0,0),none4)
+  | (_ ,(None,(None,Some handl))) => ((1,4),(Some (inr handl),(None,(Some handl,None)))) (*(1,4) = turn off yourself, turn on scheduler*)
+  | _ => ((0,0),none4)    
   end.
 
-Fixpoint projOl (V I O : Ty) (t : seq ([Times V I] + [Times V O])) : seq ([Times V I] + [O]) :=
-  match t with
-  | nil => nil
-  | x :: t' => projO x :: projOl t'
-  end.
+Definition my_f_in_sch_good (t : [my_T_in]) : [Times Nat Nat] := match t with | inl tt | inr DiskInterrupt => (0,0) | inr TimerInterrupt => (0,4) end.
+Definition my_f_in_t (t : [my_T_in]) : [ (times_Option_n 3 my_f_I) ] := match t with
+                                                                        | inl tt => (None,(Some tt,(None,None)))
+                                                                        | inr TimerInterrupt => (Some (inl TimerInterrupt),(None,(None,None)))
+                                                                        | inr DiskInterrupt => (None,(None,(None,Some DiskInterrupt))) end.
+Definition my_f_in_good (t : [my_T_in]) : [my_T_in'] := (my_f_in_sch_good t, my_f_in_t t).
+Definition my_f_out (t : [my_T_out']) := match t with
+                                         | (_,(Some p,(None,None))) => Some (inl p)
+                                         | (_,(None,(Some sys,None))) => Some (inr sys)
+                                         | _ => None
+                                         end.
 
-(* Forward: any trace of (sta f g v p) is the projIl-image of a threaded      *)
-(* list whose projOl-image is a trace of p.                                   *)
-Lemma sta_proj : forall (I O V : Ty) (p : Proc (Times V I) O) (VRel : myrel [V]) (ORel : myrel [O]) (f : [I] -> [V] -> [V]) (g : [O] -> [V] -> [V]) l v ts,
-    Trace (eqpair VRel ORel) l ts (sta f g v p) ->
-    exists t, ts = projIl t /\ Trace ORel l (projOl t) p.
+Definition f_out_dis (v : [my_T_out]) := match v with | Some (inl _) | None => False | _  => True end.
+
+Definition my_f_out_rel : myrel ([my_T_out]).
+  refine (@MyRel _
+            (fun l (v : [my_T_out]) => l = \bot /\ f_out_dis v )
+            (fun l v1 v2 => v1 = v2 \/ (l = \bot /\ f_out_dis v1 /\ f_out_dis v2))
+            _
+            _
+            _
+            _).
+  intros. con. intro. auto. intro. intros. de H.
+  intro. intros. de H. de H0. left. subst. auto. subst. eauto.
+  de H0. subst. eauto.
+  intros. de H0.
+  intros. ssa. subst. apply order_bot in H. subst. ssa.
+  intros. ssa. subst. rewrite /order in H.  rewrite lex0 in H. by apply/eqP.
+  ssa.
+  con. case. intros. eauto.
+  case. intros. subst. eauto.
+  ssa.
+Defined.
+
+Definition my_only_loop_good' := @only_loop my_T_in' my_T_out' my_f_route_good my_def process_pool_good.
+
+Definition my_only_loop_good : Proc my_T_in my_T_out .
+  eapply map. apply my_f_in_good. apply my_f_out. apply my_only_loop_good'.
+Defined.
+
+  
+
+Definition out0 x : [my_T_out'] := (Some x,(None,(None,None))).
+Definition out1 x : [my_T_out'] := (None,(Some x,(None,None))).
+Definition out2 x : [my_T_out'] := (None,(None,(Some x,None))).
+Definition out3 x : [my_T_out'] := (None,(None,(None, Some x))).
+
+(*Spec for good scheduler*)
+(*Add diskinterrupt*)
+Definition streamType' := Stream ([my_T_in'] + [my_T_out']).
+Definition newtrace'F (s : streamType') := Cons (inl (my_f_in_good (inr TimerInterrupt))) (*jump to scheduler*)
+                                             (Cons (inr ((Some (2,1)),(None,(Some NOP,None)))) (*private process does nothing, scheduler points to handler*)
+                                             (Cons (inr (out3 Nothing)) (*handler finishes, returns control to scheduler*)
+                                             (Cons (inr (out0 (3,3))) (*scheduler points to public*)
+                                             (Cons (inr (out1 GetRequest)) (*public output*)
+                                             (Cons (inl (my_f_in_good (inr DiskInterrupt)))(*disk interrupt, should NOT jump to handler*)
+                                             (Cons (inl (my_f_in_good (inr TimerInterrupt))) (*jump to scheduler*)
+                                             (Cons (inr (Some (3,1),(Some GetRequest,(None,None)))) (*public process finishes, scheduler points to handler*)
+                                             (Cons (inr (out3 Notify)) (*handler signal informs diskinterrupt was received*)
+                                             (Cons (inr (out0 (2,2))) (*scheduler points to private*)
+                                             (Cons (inr (None,(None,(Some Syscall,None)))) s)))))))))) (*private output received notification from handler, outputs new syscall*).
+
+CoFixpoint newtrace' := newtrace'F newtrace'.
+
+Lemma newtrace'_eq : newtrace' = newtrace'F newtrace'.
 Proof.
-  intros I O V p VRel ORel f g l v ts. move: p v. elim: ts.
-  - intros p v HT. exists nil. ssa.
-  - intros a ts IH p v HT. inv HT.
-    + match_dd. move: (IH _ _ H3) => [t] [Hpi] Hpo.
-      exists (inl (f i v, i) :: t). split.
-      * simpl. rewrite Hpi. done.
-      * simpl. econ. eauto. apply Hpo.
-    + match_dd. move: (IH _ _ H4) => [t] [Hpi] Hpo.
-      exists (inr o :: t). split.
-      * simpl. rewrite Hpi. done.
-      * simpl. econ. eauto. 2: apply Hpo. move: H2 => [_ HO]. apply HO.
+rewrite {1}/newtrace'.
+rewrite {1}(coseq_match (cofix newtrace' : streamType' := newtrace'F newtrace')).
+simpl.
+rewrite /newtrace'F.
+do ? f_equal.
 Qed.
 
-(* Specialisation to the NI call-site: the composite trace insert n (inl i) t  *)
-(* is EXACTLY projIl T, and projOl T is a trace of p, for one shared list T.    *)
-Lemma sta_proj_insert : forall (I O V : Ty) (p : Proc (Times V I) O) (VRel : myrel [V]) (ORel : myrel [O]) (f : [I] -> [V] -> [V]) (g : [O] -> [V] -> [V]) l v n i t,
-    Trace (eqpair VRel ORel) l (insert n (inl i) t) (sta f g v p) ->
-    exists T, insert n (inl i) t = projIl T /\ Trace ORel l (projOl T) p.
-Proof. intros. eapply sta_proj. apply H. Qed.
-
-(* A list is "threaded" from v when each stored state is the f/g-update of    *)
-(* the previous one, using the recorded input/output in that element.         *)
-Fixpoint threaded (V I O : Ty) (f : [I]->[V]->[V]) (g : [O]->[V]->[V]) (v : [V]) (t : seq ([Times V I] + [Times V O])) : Prop :=
-  match t with
-  | nil => True
-  | inl wi :: t' => fst wi = f (snd wi) v /\ threaded f g (f (snd wi) v) t'
-  | inr wo :: t' => fst wo = g (snd wo) v /\ threaded f g (g (snd wo) v) t'
-  end.
-
-(* Converse direction.  The INPUT case goes through (reduceI is exact-enough).  *)
-(* The OUTPUT case does NOT: rebuilding the sta-step uses p's ACTUAL output o', *)
-(* so the continuation is (sta f g (g o' v) p'), but `threaded` only provides   *)
-(* the suffix threaded from (g w2 v) where w2 is the RECORDED output, and       *)
-(* o' <> w2 (only rel ORel o' w2, since Trace records outputs up to rel).  The  *)
-(* concrete stuck goal:                                                         *)
-(*   H2  : rel ORel l o' w2                                                     *)
-(*   Hth : threaded f g (g w2 v) t                                             *)
-(*   |-  Trace (eqpair VRel ORel) l (projIl t) (sta f g (g o' v) p')           *)
-(* This is the SAME obstacle as before (NI not closed under reduceO): the       *)
-(* forward projection yields a *loose* list, the converse needs an *exactly*    *)
-(* threaded one, and bridging them needs NI of a reduceO-reduct.                *)
 
 
-(* ---- NI is closed under reduction (both reduceI and reduceO). ----          *)
-(* CORRECTION: reduceO IS deterministic (the earlier "non-determinism" was an   *)
-(* artifact of stating determinism with the output fixed; the full statement    *)
-(* below holds, and the map case closes because the subprocess has a unique     *)
-(* output).  Hence NI_reduceO holds, which is exactly what the rebuild needs.   *)
-Lemma reduceI_det : forall I O (p : Proc I O) i p1, reduceI p i p1 -> forall p2, reduceI p i p2 -> p1 = p2.
+Definition streamType := Stream ([my_T_in] + [my_T_out]).
+
+Definition newtraceF (s : streamType) := Cons (inl (inr TimerInterrupt))
+                                            (Cons (inr (Some (inr NOP)))
+                                             (Cons (inr None)
+                                             (Cons (inr None)
+                                             (Cons (inr (Some (inl GetRequest)))
+                                             (Cons (inl (inr DiskInterrupt))
+                                             (Cons (inl (inr TimerInterrupt))
+                                             (Cons (inr (Some (inl GetRequest)))
+                                             (Cons (inr None)
+                                             (Cons (inr None)
+                                             (Cons (inr (Some (inr Syscall))) s)))))))))).
+
+CoFixpoint newtrace := newtraceF newtrace.
+
+Lemma newtrace_eq : newtrace = newtraceF newtrace.
 Proof.
-  intros I O p i p1 H. elim: H; intros; match_dd; subst; f_equal; eauto.
+rewrite {1}/newtrace.
+rewrite {1}(coseq_match (cofix newtrace : streamType := newtraceF newtrace)).
+simpl.
+rewrite /newtraceF.
+do ? f_equal.
 Qed.
 
-Lemma reduceO_det : forall I O (p : Proc I O) o1 p1, reduceO p o1 p1 -> forall o2 p2, reduceO p o2 p2 -> o1 = o2 /\ p1 = p2.
+
+Ltac rewr ::=  (try rewrite newtrace'_eq); (try rewrite newtrace_eq); rewrite /low_p /handler /high_p /only_loop /my_only_loop_good' /my_only_loop_good /process_pool_good /good_schedulerp /my_f_coopt /scheduled_process_pool /high_p /alternate_generic /alternate_generic2 /low_p.
+
+(*spec for good scheduler*)
+Lemma newtrace'_trace : trace newtrace' my_only_loop_good'.
 Proof.
-  intros I O p o1 p1 H. elim: H; intros; match_dd;
-  repeat (match goal with
-          | [ IH : forall o2 p2, reduceO ?q o2 p2 -> _, HH : reduceO ?q _ _ |- _ ] =>
-              apply IH in HH; destruct HH
-          | [ E : (_, _) = (_, _) |- _ ] => inversion E; clear E
-          | [ H1 : reduceI ?q ?i ?a, H2 : reduceI ?q ?i ?b |- _ ] =>
-              assert (a = b) by (eapply reduceI_det; eassumption); clear H2
-          end; subst);
-  split; reflexivity.
+  pcofix CIH. 
+  bundle;left.
+  bundle;left.
+  bundle;left.
+  bundle;left.
+  bundle;left.
+  bundle;left.
+  bundle;left.
+  instantiate (1:= 0). instantiate (1:= 0). instantiate (1:= 0). simpl.
+  bundle;left.
+  bundle;left.
+  bundle;left.
+  bundle;right.
+  swi_instans. simpl. eauto.
 Qed.
 
-Lemma NI_reduceI : forall I O (IRel : myrel [I]) (ORel : myrel [O]) (p p' : Proc I O) i,
-    NI IRel ORel p -> reduceI p i p' -> NI IRel ORel p'.
+
+(*spec for good scheduler (what the world sees)*)
+Lemma newtrace_trace : trace newtrace my_only_loop_good.
 Proof.
-  intros I O IRel ORel p p' i HNI Hred l.
-  move: (HNI l) => [Hrel [Hins Hrem]]. split;[|split].
-  - intros t a a' n Hr HT.
-    have HTp2: Trace ORel l (insert n.+1 (inl a) (inl i :: t)) p. econ. apply Hred. apply HT.
-    apply (Hrel (inl i :: t) a a' n.+1 Hr) in HTp2.
-    simpl in HTp2. inv HTp2. eapply reduceI_det in Hred. 2: apply H1. subst. apply H3.
-  - intros t a n Hd HT.
-    have HTp: Trace ORel l (inl i :: t) p. econ. apply Hred. apply HT.
-    apply (Hins (inl i :: t) a n.+1 Hd) in HTp.
-    simpl in HTp. inv HTp. eapply reduceI_det in Hred. 2: apply H1. subst. apply H3.
-  - intros t a n Hd HT.
-    have HTp: Trace ORel l (insert n.+1 (inl a) (inl i :: t)) p. simpl. econ. apply Hred. apply HT.
-    apply (Hrem (inl i :: t) a n.+1 Hd) in HTp.
-    simpl in HTp. inv HTp. eapply reduceI_det in Hred. 2: apply H1. subst. apply H3.
+  pcofix CIH.
+  bundle;left.
+  bundle;left.
+  bundle;left.
+  bundle;left.
+  bundle;left.
+  bundle;left.  
+  bundle;left.
+  bundle.
+  instantiate (2:= None). simpl.
+  instantiate (1:= None). simpl. done.
+  instantiate (3:=0). simpl. reduce_once. econ.
+  reduce_tac.
+  instantiate (2:= 0). simpl.
+  reduce_once.
+  instantiate (2:= 0). simpl.
+  reduce_once.
+  simpl. reduce_once. econ.
+  reduce_tac.
+  reduce_tac.
+  reduce_tac.
+  reduce_tac.
+  left.
+  
+  bundle;left.
+  bundle;left.  
+  bundle;right.
+  swi_instans.
+  eauto.
 Qed.
 
-Lemma NI_reduceO : forall I O (IRel : myrel [I]) (ORel : myrel [O]) (p p' : Proc I O) o,
-    NI IRel ORel p -> reduceO p o p' -> NI IRel ORel p'.
-Proof.
-  intros I O IRel ORel p p' o HNI Hred l.
-  move: (HNI l) => [Hrel [Hins Hrem]]. split;[|split].
-  - intros t a a' n Hr HT.
-    have HTp: Trace ORel l (inr o :: insert n (inl a) t) p. econ. apply Hred. apply rel_refl. apply HT.
-    apply (Hrel (inr o :: t) a a' n.+1 Hr) in HTp.
-    simpl in HTp. inv HTp. eapply reduceO_det in Hred. 2: apply H1. destruct Hred. subst. assumption.
-  - intros t a n Hd HT.
-    have HTp: Trace ORel l (inr o :: t) p. econ. apply Hred. apply rel_refl. apply HT.
-    apply (Hins (inr o :: t) a n.+1 Hd) in HTp.
-    simpl in HTp. inv HTp. eapply reduceO_det in Hred. 2: apply H1. destruct Hred. subst. assumption.
-  - intros t a n Hd HT.
-    have HTp: Trace ORel l (inr o :: insert n (inl a) t) p. econ. apply Hred. apply rel_refl. apply HT.
-    apply (Hrem (inr o :: t) a n.+1 Hd) in HTp.
-    simpl in HTp. inv HTp. eapply reduceO_det in Hred. 2: apply H1. destruct Hred. subst. assumption.
-Qed.
 
-(* Structural helpers for the NI proof (both straightforward, left Admitted). *)
-Lemma projIl_insert_inv : forall (V I O : Ty) (v : [V]) (T : seq ([Times V I] + [Times V O])) n i t,
-    projIl T = insert n (inl i) t -> exists w T'', T = insert n (inl (w, i)) T'' /\ projIl T'' = t.
-Proof.
-  intros V I O v T. elim: T => [| a T' IH] n i t H.
-  - simpl in H. destruct n; simpl in H.
-    + discriminate.
-    + destruct t; try discriminate.
-      exists v, nil. split; done.
-  - destruct n.
-    + simpl in H. inversion H. subst.
-      destruct a as [[w i0] | vo].
-      * simpl in H1. inversion H1. subst.
-        exists w, T'. split; done.
-      * simpl in H1. discriminate.
-    + destruct t as [| s t']; simpl in H.
-      * discriminate.
-      * inversion H. subst.
-        have Haux := IH n i t' H2.
-        destruct Haux as [w Haux2].
-        destruct Haux2 as [T'' Haux3].
-        destruct Haux3 as [HT'' Hproj].
-        subst T'. exists w, (a :: T'' ). split.
-        -- simpl. done.
-        -- simpl. rewrite Hproj. done.
-Qed.
 
-Lemma projOl_insert : forall (V I O : Ty) n (x : [Times V I] + [Times V O]) (T : seq ([Times V I] + [Times V O])),
-    projOl (insert n x T) = insert n (projO x) (projOl T).
-Proof.
-  intros. elim: n T => [| n IH] T; destruct T; simpl; eauto.
-  by rewrite IH.
-Qed.
 
-Lemma projIl_insert : forall (V I O : Ty) n (x : [Times V I] + [Times V O]) (T : seq ([Times V I] + [Times V O])),
-    projIl (insert n x T) = insert n (projI x) (projIl T).
-Proof.
-  intros. elim: n T => [| n IH] T; destruct T; simpl; eauto.
-  by rewrite IH.
-Qed.
 
-(* ---- The converse machinery (uses NI_reduceI / NI_reduceO). ----            *)
-(* lthread v L : the stored states in L are rel-related to the f/g state-thread *)
-(* from v (a "loose" threading, which is all a real observed trace gives).      *)
-Fixpoint lthread (V I O : Ty) (VRel : myrel [V]) (f : [I]->[V]->[V]) (g : [O]->[V]->[V]) (l : level) (v : [V]) (L : seq ([Times V I] + [Times V O])) : Prop :=
-  match L with
-  | nil => True
-  | inl wi :: L' => rel VRel l (fst wi) (f (snd wi) v) /\ lthread VRel f g l (f (snd wi) v) L'
-  | inr wo :: L' => rel VRel l (fst wo) (g (snd wo) v) /\ lthread VRel f g l (g (snd wo) v) L'
-  end.
+(*Now the bad process*)
 
-Lemma lthread_stable : forall (V I O : Ty) (VRel : myrel [V]) (IRel : myrel [I]) (ORel : myrel [O]) (f : [I]->[V]->[V]) (g : [O]->[V]->[V]) l L v v',
-    fv_NI IRel VRel VRel f -> fv_NI ORel VRel VRel g ->
-    rel VRel l v v' -> lthread VRel f g l v L -> lthread VRel f g l v' L.
-Proof.
-  intros V I O VRel IRel ORel f g l L. elim: L => [|a L' IH] v v' Hf Hg Hvv' Hl; first done.
-  destruct a as [[w x]|[w x]]; simpl in *; destruct Hl as [Hw Hl]; split.
-  - eapply rel_trans. apply Hw. eapply Hf. apply rel_refl. apply Hvv'.
-  - eapply IH. apply Hf. apply Hg. 2: apply Hl. eapply Hf. apply rel_refl. apply Hvv'.
-  - eapply rel_trans. apply Hw. eapply Hg. apply rel_refl. apply Hvv'.
-  - eapply IH. apply Hf. apply Hg. 2: apply Hl. eapply Hg. apply rel_refl. apply Hvv'.
-Qed.
 
-(* The converse: a p-trace (projOl L) lifts to an sta-trace (projIl L).  At an  *)
-(* input it re-aligns p's state-component via p's clause 1 + NI_reduceI; at an  *)
-(* output it observes p's actual output and continues via NI_reduceO.           *)
-Lemma sta_conv : forall (I O V : Ty) (VRel : myrel [V]) (IRel : myrel [I]) (ORel : myrel [O]) (f : [I]->[V]->[V]) (g : [O]->[V]->[V]) l L (p : Proc (Times V I) O) v,
-    fv_NI ORel VRel VRel g -> fv_NI IRel VRel VRel f ->
-    NI (eqpair_R VRel IRel) ORel p ->
-    Trace ORel l (projOl L) p -> lthread VRel f g l v L ->
-    Trace (eqpair VRel ORel) l (projIl L) (sta f g v p).
-Proof.
-  intros I O V VRel IRel ORel f g l L. elim: L => [|a L' IH] p v Hg Hf HNI HT Hl.
-  - simpl. con.
-  - destruct a as [[w x]|[w x]]; simpl in *; destruct Hl as [Hw Hl].
-    + move: (HNI l) => [Hrel _].
-      have Hsw : rel (eqpair_R VRel IRel) l (w,x) (f x v, x) by (left; split; [apply Hw | apply rel_refl]).
-      apply (Hrel (projOl L') (w,x) (f x v, x) 0 Hsw) in HT.
-      simpl in HT. inv HT.
-      econ. econ. reflexivity. apply H1.
-      eapply IH. apply Hg. apply Hf. eapply NI_reduceI. apply HNI. apply H1. apply H3. apply Hl.
-    + inv HT.
-      econ. econ. reflexivity. apply H1.
-      split. eapply rel_trans. eapply Hg. apply H2. apply rel_refl. apply rel_sym. apply Hw. apply H2.
-      eapply IH. apply Hg. apply Hf. eapply NI_reduceO. apply HNI. apply H1. apply H4.
-      eapply lthread_stable. apply Hf. apply Hg. 2: apply Hl. eapply Hg. apply rel_sym. apply H2. apply rel_refl.
-Qed.
-
-(* Forward decomposition with the lthread invariant. *)
-Lemma sta_proj_lthread : forall (I O V : Ty) (p : Proc (Times V I) O) (VRel : myrel [V]) (IRel : myrel [I]) (ORel : myrel [O]) (f : [I] -> [V] -> [V]) (g : [O] -> [V] -> [V]) l v ts,
-    fv_NI IRel VRel VRel f -> fv_NI ORel VRel VRel g ->
-    Trace (eqpair VRel ORel) l ts (sta f g v p) ->
-    exists T, ts = projIl T /\ Trace ORel l (projOl T) p /\ lthread VRel f g l v T.
-Proof.
-  intros I O V p VRel IRel ORel f g l v ts. move: p v. elim: ts.
-  - intros p v Hf Hg HT. exists nil. ssa.
-  - intros a ts IH p v Hf Hg HT. inv HT.
-    + match_dd. move: (IH _ _ Hf Hg H3) => [T] [Hpi] [Hpo] Hlt.
-      exists (inl (f i v, i) :: T). split; [|split].
-      * simpl. rewrite Hpi. done.
-      * simpl. econ. eauto. apply Hpo.
-      * simpl. split. apply rel_refl. apply Hlt.
-    + match_dd. destruct o as [vobs oobs].
-      move: H2 => /= [HV HO].
-      move: (IH _ _ Hf Hg H4) => [T] [Hpi] [Hpo] Hlt.
-      exists (inr (vobs, oobs) :: T). split; [|split].
-      * simpl. rewrite Hpi. done.
-      * simpl. econ. eauto. apply HO. apply Hpo.
-      * simpl. split.
-        eapply rel_trans. apply rel_sym. apply HV. eapply Hg. apply HO. apply rel_refl.
-        eapply lthread_stable. apply Hf. apply Hg. 2: apply Hlt. eapply Hg. apply HO. apply rel_refl.
-Qed.
-
-(* Swapping the i-component of one input preserves lthread. *)
-Lemma lthread_swap : forall (V I O : Ty) (VRel : myrel [V]) (IRel : myrel [I]) (ORel : myrel [O]) (f : [I]->[V]->[V]) (g : [O]->[V]->[V]) l T'' n w i i' v,
-    fv_NI IRel VRel VRel f -> fv_NI ORel VRel VRel g -> rel IRel l i i' ->
-    lthread VRel f g l v (insert n (inl (w, i)) T'') ->
-    lthread VRel f g l v (insert n (inl (w, i')) T'').
-Proof.
-  intros V I O VRel IRel ORel f g l T''. elim: T'' => [|a T0 IH] n w i i' v Hf Hg Hii Hl.
-  - destruct n; simpl in *.
-    + destruct Hl as [Hw _]. split. eapply rel_trans. apply Hw. eapply Hf. apply Hii. apply rel_refl. done.
-    + done.
-  - destruct n.
-    + destruct Hl as [Hw Hl]. split.
-      * eapply rel_trans. apply Hw. eapply Hf. apply Hii. apply rel_refl.
-      * eapply lthread_stable. apply Hf. apply Hg. 2: apply Hl. eapply Hf. apply Hii. apply rel_refl.
-    + simpl in Hl |- *. destruct a as [[w2 x2]|[w2 x2]]; destruct Hl as [Hw2 Hl]; split.
-      * apply Hw2.
-      * eapply IH. apply Hf. apply Hg. apply Hii. apply Hl.
-      * apply Hw2.
-      * eapply IH. apply Hf. apply Hg. apply Hii. apply Hl.
-Qed.
-
-Lemma lthread_insert_dis : forall (V I O : Ty) (VRel : myrel [V]) (IRel : myrel [I]) (ORel : myrel [O]) (f : [I]->[V]->[V]) (g : [O]->[V]->[V]) l T n i v,
-    fv_NI IRel VRel VRel f -> fv_NI ORel VRel VRel g -> f_EP IRel VRel f -> dis IRel l i ->
-    lthread VRel f g l v T ->
-    exists w, lthread VRel f g l v (insert n (inl (w, i)) T).
-Proof.
-  intros V I O VRel IRel ORel f g l T n i v Hf Hg Hep Hdi. move: T v. elim: n => [| n' IH] T v Hlt.
-  - exists (f i v). simpl. split.
-    + apply rel_refl.
-    + eapply lthread_stable. apply Hf. apply Hg. 2: apply Hlt.
-      apply rel_sym. apply Hep. apply Hdi.
-  - destruct T as [| a' T0].
-    + exists v. simpl. done.
-    + destruct a' as [[w0 i0] | [w0 o0]]; simpl in *; destruct Hlt as [Hw0 Hlt].
-      * destruct (IH T0 (f i0 v) Hlt) as [w Hw].
-        exists w. split; assumption.
-      * destruct (IH T0 (g o0 v) Hlt) as [w Hw].
-        exists w. split; assumption.
-Qed.
-
-Lemma lthread_remove_dis : forall (V I O : Ty) (VRel : myrel [V]) (IRel : myrel [I]) (ORel : myrel [O]) (f : [I]->[V]->[V]) (g : [O]->[V]->[V]) l T'' n w i v,
-    fv_NI IRel VRel VRel f -> fv_NI ORel VRel VRel g -> f_EP IRel VRel f -> dis IRel l i ->
-    lthread VRel f g l v (insert n (inl (w, i)) T'') ->
-    lthread VRel f g l v T''.
-Proof.
-  intros V I O VRel IRel ORel f g l T'' n w i v Hf Hg Hep Hdi Hlt.
-  move: T'' v Hlt. elim: n => [| n' IH] T'' v Hlt.
-  - destruct T'' as [| a' T0]; simpl in Hlt.
-    + done.
-    + destruct Hlt as [Hw Hlt]. eapply lthread_stable. apply Hf. apply Hg. 2: apply Hlt.
-      eapply Hep. apply Hdi.
-  - destruct T'' as [| a' T0].
-    + simpl. done.
-    + destruct a' as [[w0 i0] | [w0 o0]]; simpl in Hlt |- *; destruct Hlt as [Hw0 Hlt].
-      * split; [apply Hw0 | eapply IH; eauto].
-      * split; [apply Hw0 | eapply IH; eauto].
-Qed.
-
-(* sta_NI: clause 1 (rel) is PROVED via the projection + converse approach.     *)
-(* Clauses 2 (insert disclosed) and 3 (remove) are analogous (using p's clauses *)
-(* 2/3 and f_EP) and are left admitted.                                         *)
-Lemma sta_NI : forall (I O V : Ty) (p : Proc (Times V I) O) f g v (IRel : myrel [I]) (VRel : myrel [V]) (ORel : myrel [O]),
-    fv_NI ORel VRel VRel g -> fv_NI IRel VRel VRel f -> f_EP IRel VRel f ->
-    NI (eqpair_R VRel IRel) ORel p ->
-    NI IRel (eqpair VRel ORel) (sta f g v p).
-Proof.
-  intros I O V p f g v IRel VRel ORel Hg Hf Hep Hp. rewrite /NI /NI_l. intros l. ssa.
-  - (* clause 1 (rel) -- PROVED *)
-    intros t i i' n Hii HT.
-    eapply sta_proj_lthread in HT. 2: apply Hf. 2: apply Hg.
-    move: HT => [T] [Heq] [Htp] Hlt.
-    symmetry in Heq. move/(projIl_insert_inv v) : Heq => [w] [T''] [HT' Ht''].
-    subst T. subst t.
-    rewrite projOl_insert in Htp. simpl in Htp.
-    move: (Hp l) => [Hrel _].
-    eapply (Hrel (projOl T'') (w,i) (w,i') n) in Htp;
-      last by (left; split; [apply rel_refl | apply Hii]).
-    have Hl' : lthread VRel f g l v (insert n (inl (w, i')) T'').
-    { eapply lthread_swap. apply Hf. apply Hg. apply Hii. apply Hlt. }
-    have Hfin : Trace (eqpair VRel ORel) l (projIl (insert n (inl (w, i')) T'')) (sta f g v p).
-    { eapply sta_conv. apply Hg. apply Hf. apply Hp. rewrite projOl_insert. simpl. apply Htp. apply Hl'. }
-    rewrite projIl_insert in Hfin. simpl in Hfin. apply Hfin.
-  - (* clause 2 (insert disclosed) -- PROVED *)
-    intros t i n Hdi HT.
-    eapply sta_proj_lthread in HT. 2: apply Hf. 2: apply Hg.
-    move: HT => [T] [Heq [Htp Hlt]]. subst t.
-    have [w Hw] : exists w, lthread VRel f g l v (insert n (inl (w, i)) T).
-    { eapply lthread_insert_dis; eauto. }
-    have -> : insert n (inl i) (projIl T) = projIl (insert n (inl (w, i)) T) by rewrite projIl_insert.
-    eapply sta_conv. apply Hg. apply Hf. apply Hp. 2: exact Hw.
-    rewrite projOl_insert. simpl.
-    move: (Hp l) => [_ [Hins _]]. eapply Hins. 2: apply Htp.
-    simpl. apply Hdi.
-  - (* clause 3 (remove) -- PROVED *)
-    intros t i n Hdi HT.
-    eapply sta_proj_lthread in HT. 2: apply Hf. 2: apply Hg.
-    move: HT => [T] [Heq [Htp Hlt]].
-    symmetry in Heq. move/(projIl_insert_inv v) : Heq => [w] [T''] [HT' Ht''].
-    subst T. subst t.
-    have Hl' : lthread VRel f g l v T''.
-    { eapply lthread_remove_dis; eauto. }
-    eapply sta_conv. apply Hg. apply Hf. apply Hp. 2: exact Hl'.
-    rewrite projOl_insert in Htp. simpl in Htp.
-    move: (Hp l) => [_ [_ Hrem]]. eapply Hrem; [|apply Htp].
-    simpl. apply Hdi.
-Qed.*)
-
-Inductive SwiTrace (I O : Ty) (ORel : myrel [O]) (BRel : myrel [Bool]) (l : level) : bool -> seq ([Times Bool I] + [Option O]) -> seq ([I] + [Times Bool O]) -> Prop :=
-| ST0 b : SwiTrace ORel BRel l b nil nil
-| ST1 b b' i t_swi t_p : SwiTrace ORel BRel l (xor b b') t_swi t_p -> SwiTrace ORel BRel l b (inl (b', i) :: t_swi) (inl i :: t_p)
-| ST2_false o t_swi t_p : rel (eqmaybe_swi ORel BRel) l None o -> SwiTrace ORel BRel l false t_swi t_p -> SwiTrace ORel BRel l false (inr o :: t_swi) t_p
-| ST2_true b_out o o_obs t_swi t_p : rel (eqmaybe_swi ORel BRel) l (Some o) o_obs -> SwiTrace ORel BRel l (negb b_out) t_swi t_p -> SwiTrace ORel BRel l true (inr o_obs :: t_swi) (inr (b_out, o) :: t_p).
-
-Lemma swi_trace : forall (I O : Ty) (p : Proc I (Times Bool O)) (ORel : myrel [O]) (BRel : myrel [Bool]) l b t,
-    Trace (eqmaybe_swi ORel BRel) l t (swi b p) ->
-    exists t', Trace (eqpair_LR BRel ORel) l t' p /\ SwiTrace ORel BRel l b t t'.
-Proof.
-  intros I O p ORel BRel l b t HT.
-  move: p b HT.
-  elim: t => [| a t IH] p b HT.
-  - exists nil. split.
-    + con.
-    + con.
-  - inv HT.
-    + destruct i as [b' i_in]. dependent destruction H1.
-      edestruct (IH p'0 (xor b b') H3) as [t' [Htrace Hswi]].
-      exists (inl i_in :: t'). split.
-      * econstructor; eauto.
-      * econstructor; eauto.
-    + dependent destruction H1.
-      * edestruct (IH p false H4) as [t' [Htrace Hswi]].
-        exists t'. split.
-        { exact Htrace. }
-        { eapply ST2_false; eauto. }
-      * edestruct (IH p'0 (negb b0) H4) as [t' [Htrace Hswi]].
-        exists (inr (b0, o0) :: t'). split.
-        { econstructor. exact H1. apply rel_refl. exact Htrace. }
-        { eapply ST2_true; eauto. }
-Qed.
-
-Lemma swi_trace_insert : forall (I O : Ty) (ORel : myrel [O]) (BRel : myrel [Bool]) l b t t' n (i : bool * [I]),
-    i.1 = false ->
-    SwiTrace ORel BRel l b (insert n (inl i) t) t' ->
-    exists n' t'', t' = insert n' (inl i.2) t'' /\ SwiTrace ORel BRel l b t t''.
-Proof.
-  intros I O ORel BRel l b t t' n i Hi1 H.
-  elim: t b t' n H => [| a t IH] b t' n H.
-  - ssa. destruct n; simpl in H.
-    + inv H. match goal with | Hswi : SwiTrace _ _ _ _ _ _ |- _ => inversion Hswi; subst end.
-      exists 0, nil. split; [done | constructor].
-    + inv H. exists 1, nil. split; [done | constructor].
-  - ssa. destruct n; simpl in H.
-    + inv H. exists 0, t_p. split; [done |].
-      simpl in Hi1. rewrite Hi1 xorFalse in H4. exact H4.
-    + inv H.
-      * ssa. match goal with | Hswi : SwiTrace _ _ _ _ _ _ |- _ => destruct (IH _ _ _ Hswi) as [n' [t'' [-> Hswi2]]] end.
-        exists n'.+1, (inl i0 :: t''). split; [done |].
-        constructor. exact Hswi2.
-      * ssa. match goal with | Hswi : SwiTrace _ _ _ _ _ _ |- _ => destruct (IH _ _ _ Hswi) as [n' [t'' [-> Hswi2]]] end.
-        exists n', t''. split; [done |].
-        eapply ST2_false; eauto.
-      * ssa. match goal with | Hswi : SwiTrace _ _ _ _ _ _ |- _ => destruct (IH _ _ _ Hswi) as [n' [t'' [-> Hswi2]]] end.
-        exists n'.+1, (inr (b_out, o) :: t''). split; [done |].
-        eapply ST2_true; eauto.
-Qed.
-
-Lemma swi_trace_insert_conv : forall (I O : Ty) (ORel : myrel [O]) (BRel : myrel [Bool]) l b t t_p n (i : bool * [I]),
-    aware BRel true l ->
-    dis BRel l i.1 ->
-    SwiTrace ORel BRel l b t t_p ->
-    exists n', SwiTrace ORel BRel l b (insert n (inl i) t) (insert n' (inl i.2) t_p).
-Proof.
-  intros I O ORel BRel l b t t_p n [b_in i_in] Haware Hdis Hswi.
-  have Hb_in : b_in = false.
-  { destruct b_in; [| done].
-    have Hrefl : rel BRel l true true by apply: rel_refl.
-    have [_ Hnd] := Haware true Hrefl.
-    contradiction. }
-  rewrite Hb_in.
-  elim: t b t_p n Hswi => [| a t IH] b t_p n Hswi.
-  - inv Hswi. destruct n; simpl.
-    + exists 0. repeat constructor.
-    + exists 1. constructor.
-  - inv Hswi.
-    + destruct n; simpl.
-      * exists 0. apply ST1. apply ST1. rewrite xorFalse.
-        match goal with | H : SwiTrace _ _ _ _ t _ |- _ => exact H end.
-      * ssa. match goal with | H : SwiTrace _ _ _ _ t _ |- _ => destruct (IH _ _ n H) as [n' Hswi_ih] end.
-        exists n'.+1. constructor. exact Hswi_ih.
-    + destruct n; simpl.
-      * exists 0. repeat constructor; eauto.
-      * ssa. match goal with | H : SwiTrace _ _ _ _ t _ |- _ => destruct (IH _ _ n H) as [n' Hswi_ih] end.
-        exists n'. eapply ST2_false; eauto.
-    + destruct n; simpl.
-      * exists 0. repeat constructor; eauto.
-      * ssa. match goal with | H : SwiTrace _ _ _ _ t _ |- _ => destruct (IH _ _ n H) as [n' Hswi_ih] end.
-        exists n'.+1. eapply ST2_true; eauto.
-Qed.
-
-Lemma swi_trace_swap : forall (I O : Ty) (ORel : myrel [O]) (BRel : myrel [Bool]) l b t t_p n (i i' : bool * [I]),
-    i.1 = i'.1 ->
-    SwiTrace ORel BRel l b (insert n (inl i) t) t_p ->
-    exists n' t_p', t_p = insert n' (inl i.2) t_p' /\ SwiTrace ORel BRel l b (insert n (inl i') t) (insert n' (inl i'.2) t_p').
-Proof.
-  intros I O ORel BRel l b t t_p n [b_in i_in] [b_in' i_in'] Heq Hswi.
-  simpl in Heq.
-  elim: t b t_p n Hswi => [| a t IH] b t_p n Hswi.
-  - ssa. destruct n; simpl in Hswi.
-    + inv Hswi. match goal with | Hswi' : SwiTrace _ _ _ _ _ _ |- _ => inversion Hswi'; subst end.
-      exists 0, nil. split; [done |].
-      try rewrite Heq. repeat constructor.
-    + inv Hswi. exists 1, nil. split; [done | constructor].
-  - ssa. destruct n; simpl in Hswi.
-    + inv Hswi. exists 0, t_p0. split; [done |].
-      try rewrite Heq. repeat constructor. exact H4.
-    + inv Hswi.
-      * ssa. match goal with | Hswi' : SwiTrace _ _ _ _ _ _ |- _ => destruct (IH _ _ _ Hswi') as [n' [t_p' [-> Hswi2]]] end.
-        exists n'.+1, (inl i :: t_p'). split; [done |].
-        constructor. exact Hswi2.
-      * ssa. match goal with | Hswi' : SwiTrace _ _ _ _ _ _ |- _ => destruct (IH _ _ _ Hswi') as [n' [t_p' [-> Hswi2]]] end.
-        exists n', t_p'. split; [done |].
-        eapply ST2_false; eauto.
-      * ssa. match goal with | Hswi' : SwiTrace _ _ _ _ _ _ |- _ => destruct (IH _ _ _ Hswi') as [n' [t_p' [-> Hswi2]]] end.
-        exists n'.+1, (inr (b_out, o) :: t_p'). split; [done |].
-        eapply ST2_true; eauto.
-Qed.
-
-Lemma swi_trace_remove : forall (I O : Ty) (ORel : myrel [O]) (BRel : myrel [Bool]) l b t t_p n (i : bool * [I]),
-    aware BRel true l ->
-    dis BRel l i.1 ->
-    SwiTrace ORel BRel l b (insert n (inl i) t) t_p ->
-    exists n' t_p', t_p = insert n' (inl i.2) t_p' /\ SwiTrace ORel BRel l b t t_p'.
-Proof.
-  intros I O ORel BRel l b t t_p n [b_in i_in] Haware Hdis Hswi.
-  have Hb_in : b_in = false.
-  { destruct b_in; [| done].
-    have Hrefl : rel BRel l true true by apply: rel_refl.
-    have [_ Hnd] := Haware true Hrefl.
-    contradiction. }
-  rewrite Hb_in in Hswi.
-  elim: t b t_p n Hswi => [| a t IH] b t_p n Hswi.
-  - ssa. destruct n; simpl in Hswi.
-    + inv Hswi. match goal with | Hswi' : SwiTrace _ _ _ _ _ _ |- _ => inversion Hswi'; subst end.
-      exists 0, nil. split; [done | constructor].
-    + inv Hswi. exists 1, nil. split; [done | constructor].
-  - ssa. destruct n; simpl in Hswi.
-    + inv Hswi. exists 0, t_p0. split; [done |].
-      rewrite xorFalse in H4. exact H4.
-    + inv Hswi.
-      * ssa. match goal with | Hswi' : SwiTrace _ _ _ _ _ _ |- _ => destruct (IH _ _ _ Hswi') as [n' [t_p' [-> Hswi2]]] end.
-        exists n'.+1, (inl i :: t_p'). split; [done |].
-        constructor. exact Hswi2.
-      * ssa. match goal with | Hswi' : SwiTrace _ _ _ _ _ _ |- _ => destruct (IH _ _ _ Hswi') as [n' [t_p' [-> Hswi2]]] end.
-        exists n', t_p'. split; [done |].
-        eapply ST2_false; eauto.
-      * ssa. match goal with | Hswi' : SwiTrace _ _ _ _ _ _ |- _ => destruct (IH _ _ _ Hswi') as [n' [t_p' [-> Hswi2]]] end.
-        exists n'.+1, (inr (b_out, o) :: t_p'). split; [done |].
-        eapply ST2_true; eauto.
-Qed.
-
-Lemma swi_conv : forall (I O : Ty) (p : Proc I (Times Bool O)) (ORel : myrel [O]) (BRel : myrel [Bool]) l b t t_p,
-    aware BRel true l ->
-    Trace (eqpair_LR BRel ORel) l t_p p -> SwiTrace ORel BRel l b t t_p -> Trace (eqmaybe_swi ORel BRel) l t (swi b p).
-Proof.
-  intros I O p ORel BRel l b t t_p Haware HT Hswi.
-  move: p HT.
-  elim: Hswi.
-  - intros b' p HT. simpl. con.
-  - intros b' b'' i t_swi t_p' Hswi IH p HT.
-    inv HT.
-    econstructor; [eapply reduce_swiI; eauto | eapply IH; exact H3].
-  - intros o t_swi t_p' Hrel Hswi IH p HT.
-    econstructor; [eapply reduce_swiO; eauto | exact Hrel | eapply IH; exact HT].
-  - intros b_out o o_obs t_swi t_p' Hrel Hswi IH p HT.
-    inv HT.
-    destruct o' as [b_out' o''].
-    destruct H2 as [Hb Ho].
-    simpl in Hb, Ho.
-    have Ho' : rel (eqmaybe_swi ORel BRel) l (Some o'') (Some o) by exact Ho.
-    econstructor.
-    + eapply reduce_swiO2; [reflexivity | exact H1].
-    + eapply rel_trans; [exact Ho' | exact Hrel].
-    + destruct b_out', b_out.
-      * eapply IH; exact H4.
-      * move: (Haware false Hb) => [H_eq _]. discriminate H_eq.
-      * move: (rel_sym Hb) => Hb_sym. move: (Haware false Hb_sym) => [H_eq _]. discriminate H_eq.
-      * eapply IH; exact H4.
-Qed.
+(*
+private on ->(?tI)
+private on, scheduler on ->(!public)
+public on ->(?dI)
+public on, handler on -> !(public,notification)
+public on ->(?tI)
+scheduler on, public on ->(!handler)
+handler on ->(!notification)
+scheduler on ->(!private)
+...
+ *)
+Definition good_schedulerp :  Proc (Sum TInterrupt THandlerOutput) (Times Nat Nat). (*handlerflag, processflag*)
+  eapply map. apply id. instantiate (1:= Times (Times Bool Bool) Unit).
+  exact (fun o => match fst o with | (true,false) => (3,1) | (true,true) => (2,1) | (false,true) => (3,3) | (false,false) => (2,2) end ).
+  eapply (@sta _ _ _). exact (fun ih bb => match ih with | inl TimerInterrupt => (true,~~ (snd bb))
+                                                         | inr _ => (false,snd bb)
+                                                         | _ => bb          
+                                           end).
+  exact (fun _ bb => bb).
+  exact (false,false).
+  eapply out. con.
+Defined.
